proof/invariant-abstract/DetSchedSchedule_AI.thy
@@ -33,9 +33,13 @@ lemma hoare_drop_assertion:
   shows "\<lbrace>Q\<rbrace> f \<lbrace>R\<rbrace>"
   by (wpsimp wp: assms)
 
-lemma do_machine_op_cur_sc_chargeable[wp]:
-  "do_machine_op f \<lbrace>cur_sc_chargeable\<rbrace>"
-  unfolding do_machine_op_def by wpsimp
+lemma valid_sched_schedulable_ipc_queues[elim!]:
+  "valid_sched s \<Longrightarrow> schedulable_ipc_queues s"
+  by (simp add: valid_sched_def)
+
+definition
+  cur_thread_on_preemption :: "'z::state_ext state \<Rightarrow> bool" where
+  "cur_thread_on_preemption \<equiv> ct_not_queued and ct_not_in_release_q and cur_sc_chargeable"
 
 lemma as_user_cur_sc_chargeable[wp]:
   "as_user f d \<lbrace>cur_sc_chargeable\<rbrace>"
@@ -424,7 +428,7 @@ lemma tcb_release_remove_wp[valid_sched_wp]:
   by (wpsimp simp: tcb_release_remove_def obj_at_def)
 
 lemma tcb_release_remove_valid_sched_misc[wp]:
-  "tcb_release_remove t \<lbrace>\<lambda>s. P (cur_time s) (cur_domain s) (cur_thread s) (idle_thread s)
+  "tcb_release_remove t \<lbrace>\<lambda>s. P (consumed_time s) (cur_sc s) (cur_time s) (cur_domain s) (cur_thread s) (idle_thread s)
                                (ready_queues s) (scheduler_action s) (last_machine_time_of s)
                                (kheap s)\<rbrace>"
   by (wpsimp wp: valid_sched_wp)
@@ -875,7 +879,7 @@ lemma reschedule_required_ct_not_queued[wp]:
   by (wpsimp wp: valid_sched_wp simp: valid_sched_wpsimps scheduler_act_not_def)
 
 lemma reschedule_required_scheduler_act_sane[wp]:
-  "\<lbrace>scheduler_act_sane\<rbrace> reschedule_required \<lbrace>\<lambda>_. scheduler_act_sane\<rbrace>"
+  "\<lbrace>\<top>\<rbrace> reschedule_required \<lbrace>\<lambda>_. scheduler_act_sane\<rbrace>"
   by (wpsimp wp: valid_sched_wp simp: valid_sched_wpsimps)
 
 \<comment> \<open>test_reschedule\<close>
@@ -1105,12 +1109,6 @@ lemma sts_obj_at_impossible'':
   apply (rule iffI, erule assms)
   apply (drule_tac st="tcb_state tcb" in assms, simp)
   done
-
-(* FIXME: move to replace set_thread_state_bound_sc_tcb_at in IpcCancel_AI *)
-lemma set_thread_state_bound_sc_tcb_at[wp]:
-  "set_thread_state t ts \<lbrace>\<lambda>s. N (bound_sc_tcb_at P t' s)\<rbrace>"
-  apply (wpsimp simp: set_thread_state_def wp: set_object_wp)
-  by (clarsimp simp: get_tcb_ko_at pred_tcb_at_def obj_at_def elim!: rsubst[of N])
 
 (* FIXME: redundant? remove? It's a bit slow without the intermediate lemmas. *)
 (* While it may be redundant, it is convenient to use in some places. *)
@@ -1404,63 +1402,6 @@ crunch ct_sched_act_not[wp]: set_thread_state "\<lambda>s. scheduler_act_not (cu
    simp: crunch_simps
    ignore: set_scheduler_action)
 
-\<comment> \<open>set_tcb_obj_ref\<close>
-  for valid_ep_q[wp]: valid_ep_q
-  and valid_ntfn_q[wp]: valid_ntfn_q
-lemma bound_sc_kh_budget_conditions_equiv:
-  "active_sc_tcb_at_kh t kh = (\<exists>scp. bound_sc_tcb_at_kh (\<lambda>ko. ko = Some scp) t kh \<and> test_sc_refill_max_kh scp kh)"
-  "budget_ready_kh curtime t kh = (\<exists>scp. bound_sc_tcb_at_kh (\<lambda>ko. ko = Some scp) t kh \<and> refill_ready_kh curtime scp 0 kh)"
-  "budget_sufficient_kh t kh = (\<exists>scp. bound_sc_tcb_at_kh (\<lambda>ko. ko = Some scp) t kh \<and> refill_sufficient_kh scp kh)"
-  unfolding bound_sc_tcb_at_kh_def obj_at_kh_def active_sc_tcb_at_kh_def
-  by fastforce+
-
-lemma bound_sc_budget_conditions_equiv:
-  "active_sc_tcb_at t s = (\<exists>scp. bound_sc_tcb_at (\<lambda>ko. ko = Some scp) t s \<and> test_sc_refill_max scp s)"
-  "budget_ready t s = (\<exists>scp. bound_sc_tcb_at (\<lambda>ko. ko = Some scp) t s \<and> is_refill_ready scp 0 s)"
-  "budget_sufficient t s = (\<exists>scp. bound_sc_tcb_at (\<lambda>ko. ko = Some scp) t s \<and> is_refill_sufficient scp 0 s)"
-  unfolding bound_sc_tcb_at_kh_def obj_at_kh_def active_sc_tcb_at_defs
-  by fastforce+
-
-lemma kh_budget_conditions_kheap_update_const:
-  "t \<noteq> t' \<Longrightarrow>
-   bound_sc_tcb_at_kh P t (\<lambda>a. if a = t' then X else kheap s a)
-   = bound_sc_tcb_at_kh P t (kheap s)"
-  "t \<noteq> t' \<Longrightarrow>
-   test_sc_refill_max_kh t (\<lambda>a. if a = t' then X else kheap s a)
-   = test_sc_refill_max_kh t (kheap s)"
-  "t \<noteq> t' \<Longrightarrow>
-   refill_sufficient_kh t (\<lambda>a. if a = t' then X else kheap s a)
-   = refill_sufficient_kh t (kheap s)"
-  "t \<noteq> t' \<Longrightarrow>
-   refill_ready_kh ct t k (\<lambda>a. if a = t' then X else kheap s a)
-   = refill_ready_kh ct t k (kheap s)"
-  unfolding bound_sc_tcb_at_kh_def obj_at_kh_def test_sc_refill_max_kh_def refill_sufficient_kh_def
-  by (fastforce simp: refill_ready_kh_def)+
-
-lemma set_thread_state_ct_valid_ntfn_q:
-  "\<lbrace> valid_ntfn_q and (\<lambda>s. thread = cur_thread s)\<rbrace> set_thread_state thread ts \<lbrace> \<lambda>_. valid_ntfn_q \<rbrace>"
-  apply (wpsimp simp: set_thread_state_def set_object_def wp: get_object_wp)
-  apply (clarsimp simp: valid_ntfn_q_def dest!: get_tcb_SomeD split: option.splits)
-  apply (drule_tac x=p in spec)
-  apply (rename_tac ko; case_tac ko; clarsimp)
-  apply (drule_tac x=t in bspec, simp)
-  apply (rule conjI)
-   apply (elim conjE disjE)
-    apply (clarsimp simp: bound_sc_tcb_at_kh_if_split)
-   apply (intro disjI2; intro conjI)
-     apply (clarsimp simp: bound_sc_kh_budget_conditions_equiv bound_sc_budget_conditions_equiv(1))
-     apply (rule_tac x=scp in exI)
-     apply (subst kh_budget_conditions_kheap_update_const, simp, subst kh_budget_conditions_kheap_update_const, clarsimp simp: test_sc_refill_max_def, clarsimp)
-    apply (clarsimp simp: bound_sc_kh_budget_conditions_equiv bound_sc_budget_conditions_equiv(3))
-    apply (rule_tac x=scp in exI)
-    apply (subst kh_budget_conditions_kheap_update_const, simp, subst kh_budget_conditions_kheap_update_const, clarsimp simp: is_refill_sufficient_def obj_at_def, clarsimp)
-   apply (clarsimp simp: bound_sc_kh_budget_conditions_equiv bound_sc_budget_conditions_equiv(2))
-   apply (rule_tac x=scp in exI)
-   apply (subst kh_budget_conditions_kheap_update_const, simp, subst kh_budget_conditions_kheap_update_const, clarsimp simp: is_refill_ready_def obj_at_def, clarsimp)
-  apply (clarsimp simp: st_tcb_at_kh_if_split)
-  done
-
-
 (* FIXME: move to KHeap_AI *)
 lemma set_tcb_obj_ref_pred_tcb_at:
   assumes "\<And>tcb. proj (tcb_to_itcb (f (\<lambda>_. v) tcb)) = proj (tcb_to_itcb tcb)"
@@ -1489,7 +1430,7 @@ lemma set_tcb_obj_ref_valid_sched_except_tcb_heap[wp]:
 lemma set_tcb_obj_ref_valid_sched_except_tcb_scp_heap:
   assumes "\<And>tcb. tcb_state (f (\<lambda>_. v) tcb) = tcb_state tcb"
   assumes "\<And>tcb. etcb_of (f (\<lambda>_. v) tcb) = etcb_of tcb"
-  shows "set_tcb_obj_ref f ref v \<lbrace>\<lambda>s. P (cur_time s) (cur_domain s) (cur_thread s) (idle_thread s)
+  shows "set_tcb_obj_ref f ref v \<lbrace>\<lambda>s. P (consumed_time s) (cur_sc s) (cur_time s) (cur_domain s) (cur_thread s) (idle_thread s)
                                         (ready_queues s) (release_queue s) (scheduler_action s)
                                         (last_machine_time_of s) (etcbs_of s)
                                         (tcb_sts_of s) (scs_of s)\<rbrace>"
@@ -1744,34 +1685,31 @@ lemma set_tcb_active_sc_tcb_at_const:
   set_tcb_obj_ref f ref ntfn \<lbrace>(\<lambda>s. Q (active_sc_tcb_at t s))::det_state \<Rightarrow> _\<rbrace>"
   apply (wpsimp wp: set_tcb_obj_ref_wp)
   apply (erule back_subst[where P=Q])
-  apply (clarsimp simp: active_sc_tcb_at_defs cong: conj_cong)
-  apply (fastforce)
-  done
+  apply (clarsimp simp: vs_all_heap_simps obj_at_def cong: conj_cong)
+  by auto
 
 lemma set_sc_active_sc_tcb_at_const:
   "\<forall>sc. sc_refill_max (f (\<lambda>y. ntfn) sc) = sc_refill_max (sc) \<Longrightarrow>
   set_sc_obj_ref f ref ntfn \<lbrace>(\<lambda>s. Q (active_sc_tcb_at t s))::det_state \<Rightarrow> _\<rbrace>"
   apply (wpsimp wp: set_sc_obj_ref_wp)
   apply (erule back_subst[where P=Q])
-  apply (clarsimp simp: active_sc_tcb_at_defs cong: conj_cong)
-  apply (fastforce)
-  done
+  apply (clarsimp simp: vs_all_heap_simps obj_at_def cong: conj_cong)
+  by auto
 
 lemma set_tcb_budget_sufficient_const:
   "\<forall>tcb. tcb_sched_context (f (\<lambda>a. ntfn) tcb) = tcb_sched_context tcb \<Longrightarrow>
   set_tcb_obj_ref f ref ntfn \<lbrace>(\<lambda>s. Q (budget_sufficient t s))::det_state \<Rightarrow> _\<rbrace>"
   apply (wpsimp wp: set_tcb_obj_ref_wp)
   apply (erule back_subst[where P=Q])
-  apply (clarsimp simp: budget_sufficient_defs cong: conj_cong)
-  apply (fastforce)
-  done
+  apply (clarsimp simp: vs_all_heap_simps obj_at_def  cong: conj_cong)
+  by auto
 
 lemma set_sc_budget_sufficient_const:
   "\<forall>sc. sc_refills (f (\<lambda>y. ntfn) sc) = sc_refills (sc) \<Longrightarrow>
   set_sc_obj_ref f ref ntfn \<lbrace>(\<lambda>s. Q (budget_sufficient t s))::det_state \<Rightarrow> _\<rbrace>"
   apply (wpsimp wp: set_sc_obj_ref_wp)
   apply (erule back_subst[where P=Q])
-  apply (clarsimp simp: budget_sufficient_defs cong: conj_cong)
+  apply (clarsimp simp: vs_all_heap_simps obj_at_def  cong: conj_cong)
   apply (fastforce)
   done
 
@@ -1780,7 +1718,7 @@ lemma set_tcb_obj_ref_budget_ready_const:
   set_tcb_obj_ref f ref ntfn \<lbrace>(\<lambda>s. Q (budget_ready t s))::det_state \<Rightarrow> _\<rbrace>"
   apply (wpsimp wp: set_tcb_obj_ref_wp)
   apply (erule back_subst[where P=Q])
-  apply (clarsimp simp: budget_ready_defs cong: conj_cong)
+  apply (clarsimp simp: vs_all_heap_simps obj_at_def  cong: conj_cong)
   apply (fastforce)
   done
 
@@ -1789,26 +1727,9 @@ lemma set_sc_obj_ref_budget_ready_const:
   set_sc_obj_ref f ref ntfn \<lbrace>(\<lambda>s. Q (budget_ready t s))::det_state \<Rightarrow> _\<rbrace>"
   apply (wpsimp wp: set_sc_obj_ref_wp)
   apply (erule back_subst[where P=Q])
-  apply (clarsimp simp: budget_ready_defs cong: conj_cong)
+  apply (clarsimp simp: vs_all_heap_simps obj_at_def refills_ready_def cong: conj_cong)
   apply (fastforce)
   done
-
-lemma set_tcb_obj_ref_valid_ntfn_q_const:
-  "\<forall>tcb. tcb_state (f (\<lambda>y. ntfn) tcb) = tcb_state (tcb) \<and>
-         tcb_sched_context (f (\<lambda>a. ntfn) tcb) = tcb_sched_context tcb \<Longrightarrow>
-   set_tcb_obj_ref f ref ntfn \<lbrace>valid_ntfn_q::det_state \<Rightarrow> _\<rbrace>"
-  by (wpsimp wp: valid_ntfn_q_lift set_tcb_obj_ref_obj_at_const set_tcb_pred_tcb_const hoare_vcg_disj_lift set_tcb_active_sc_tcb_at_const set_tcb_budget_sufficient_const
-                 set_tcb_obj_ref_budget_ready_const)
-
-lemma set_sc_obj_ref_valid_ntfn_q_const:
-  "\<forall>sc. sc_refills (f (\<lambda>a. ntfn) sc) = sc_refills sc
-        \<and> sc_refill_max (f (\<lambda>y. ntfn) sc) = sc_refill_max (sc) \<Longrightarrow>
-  set_sc_obj_ref f ref ntfn \<lbrace>valid_ntfn_q::det_state \<Rightarrow> _\<rbrace>"
-  by (wpsimp wp: valid_ntfn_q_lift set_sc_obj_ref_obj_at_const set_tcb_pred_tcb_const hoare_vcg_disj_lift set_sc_active_sc_tcb_at_const
-                 set_sc_budget_sufficient_const set_sc_obj_ref_budget_ready_const)
-
-  "set_tcb_obj_ref tcb_bound_notification_update ref ntfn \<lbrace>valid_ntfn_q::det_state \<Rightarrow> _\<rbrace>"
-  by (wpsimp wp: set_tcb_obj_ref_valid_ntfn_q_const)
 
 lemma set_tcb_sc_update_bound_sc_obj_tcb_at:
   "\<lbrace>\<lambda>s. (tptr \<noteq> t \<longrightarrow> bound_sc_obj_tcb_at (P (cur_time s)) t s)
@@ -2400,6 +2321,11 @@ locale DetSchedSchedule_AI =
             (\<lambda>s. scheduler_action s = resume_cur_thread)\<rbrace>
           arch_perform_invocation i
           \<lbrace>\<lambda>_. valid_sched :: 'state_ext state \<Rightarrow> _\<rbrace>"
+  (* FIXME: slim down these preconditions if possible, current preconditions are an estimate *)
+  assumes arch_perform_invocation_cur_sc_chargeable[wp]:
+    "\<And>i. \<lbrace>invs and cur_sc_chargeable and valid_arch_inv i\<rbrace>
+          arch_perform_invocation i
+          \<lbrace>\<lambda>_. cur_sc_chargeable :: 'state_ext state \<Rightarrow> _\<rbrace>"
   (* FIXME: Might not be necessary *)
   assumes arch_perform_invocation_misc[wp]:
     "\<And>i P. arch_perform_invocation i
@@ -2448,10 +2374,6 @@ locale DetSchedSchedule_AI =
   assumes arch_post_cap_deletion_budget_sufficient[wp] :
     "\<And>c Q t. arch_post_cap_deletion c \<lbrace>(\<lambda>s. Q (budget_sufficient t s)):: det_state \<Rightarrow> _\<rbrace>"
     "\<And>P c. arch_post_cap_deletion c \<lbrace>(\<lambda>s. P (release_queue s))::det_state \<Rightarrow> _\<rbrace>"
-  assumes arch_post_cap_deletion_valid_ntfn_q[wp] :
-    "\<And>P c. arch_post_cap_deletion c \<lbrace>valid_ntfn_q ::det_state \<Rightarrow> _\<rbrace>"
-  assumes arch_post_cap_deletion_valid_ep_q[wp] :
-    "\<And>P c. arch_post_cap_deletion c \<lbrace>valid_ep_q ::det_state \<Rightarrow> _\<rbrace>"
   assumes arch_post_cap_deletion_cur_thread[wp] :
     "\<And>P c. arch_post_cap_deletion c \<lbrace>(\<lambda>s. P (cur_thread s))::det_state \<Rightarrow> _\<rbrace>"
   assumes update_time_stamp_valid_machine_time[wp]:
@@ -2620,10 +2542,6 @@ lemma guarded_switch_to_valid_sched_misc[wp]:
 crunches switch_to_thread
   for valid_ready_qs[wp]: "valid_ready_qs::'state_ext state \<Rightarrow> _"
   (ignore: tcb_sched_action wp: hoare_drop_imp tcb_sched_dequeue_valid_ready_qs)
-
-lemma arch_perform_invocation_scheduler_act_sane[wp]:
-  "arch_perform_invocation iv \<lbrace>scheduler_act_sane :: det_state \<Rightarrow> _\<rbrace>"
-  by (wps, wpsimp)
 
 end
 
@@ -3114,12 +3032,6 @@ lemma set_refills_budget_ready_wp:
                   cong: conj_cong)
   by fastforce
 
-                      has_budget_kh t (cur_time s) (kheap s)))"
-  apply (clarsimp simp: valid_ep_q_def obj_at_def simple_obj_at_def split: option.splits)
-  apply (intro iffI; clarsimp)
-  apply (drule_tac x=p and y="Endpoint obj" in spec2, simp)
-  apply (case_tac x2; fastforce)
-  done
 
 abbreviation choose_thread_spec where
   "choose_thread_spec s \<equiv> choose_thread_spec_2 (cur_domain s) (cur_time s) (idle_thread s)
@@ -4164,6 +4076,19 @@ lemma unbind_notification_valid_sched[wp]:
   "unbind_notification ntfnptr \<lbrace>valid_sched_pred_strong P\<rbrace>"
   by (wpsimp simp: unbind_notification_def wp: get_tcb_obj_ref_wp)
 
+lemma sched_context_unbind_tcb_valid_sched_misc[wp]:
+  "sched_context_unbind_tcb sc_ptr
+   \<lbrace>\<lambda>s. P (consumed_time s) (cur_sc s) (cur_time s) (cur_domain s) (cur_thread s) (idle_thread s)
+          (last_machine_time_of s) (etcbs_of s) (tcb_sts_of s) \<rbrace>"
+  by (wpsimp simp: sched_context_unbind_tcb_def
+               wp: hoare_drop_imp hoare_vcg_all_lift set_tcb_sched_context_valid_sched_except_tcb_scp_heap)
+
+lemma unbind_from_sc_valid_sched_misc[wp]:
+  "unbind_from_sc tcb_ptr
+   \<lbrace>\<lambda>s. P (consumed_time s) (cur_sc s) (cur_time s) (cur_domain s) (cur_thread s) (idle_thread s)
+          (last_machine_time_of s) (etcbs_of s) (tcb_sts_of s) \<rbrace>"
+  by (wpsimp simp: unbind_from_sc_def wp: hoare_drop_imp hoare_vcg_all_lift)
+
 lemma tcb_release_remove_not_in_release_q':
   "tcb_release_remove thread \<lbrace>not_in_release_q t\<rbrace>"
   by (wpsimp simp: tcb_release_remove_def not_in_release_q_def tcb_sched_dequeue_def)
@@ -4867,40 +4792,6 @@ lemma reply_remove_tcb_valid_sched:
   apply (wpsimp wp: reply_unlink_tcb_valid_sched get_sk_obj_ref_wp)
   done
 
-lemma has_budget_def2:
-  "has_budget t s = has_budget_kh t (cur_time s) (kheap s)"
-  by (clarsimp simp: has_budget_def)
-
-lemma valid_ntfn_q_def2:
-  "(valid_ntfn_q :: det_state \<Rightarrow> _) s =
-   ((\<forall>tp np. ntfn_at_pred (\<lambda>ntfn. tp \<in> set (ntfn_queue (ntfn))) np s \<longrightarrow>
-    tp \<noteq> cur_thread s \<and>
-    tp \<noteq> idle_thread s \<and>
-    has_budget tp s \<and>
-    st_tcb_at (\<lambda>ts. ts = BlockedOnNotification np) tp s))"
-  unfolding valid_ntfn_q_def
-  apply (rule iffI; clarsimp)
-   apply (drule_tac x=np in spec; clarsimp simp: simple_obj_at_def has_budget_def2)
-  apply (clarsimp split: option.splits)
-  apply (case_tac x2; clarsimp)
-   apply (drule_tac x=t and y = p in spec2)
-   apply (clarsimp simp: has_budget_def2 simple_obj_at_def)
-  done
-
-lemma set_ntfn_obj_ref_valid_ntfn_q:
-  "\<forall>ntfn. ntfn_queue ((f (\<lambda>y. ep) ntfn)) = ntfn_queue ((ntfn)) \<Longrightarrow>
-  \<lbrace>valid_ntfn_q\<rbrace> set_ntfn_obj_ref f ptr ep \<lbrace>\<lambda>rv. valid_ntfn_q :: det_state \<Rightarrow> _\<rbrace>"
-  apply (rule hoare_weaken_pre)
-  apply (subst valid_ntfn_q_def2)
-  apply (wpsimp wp: hoare_vcg_all_lift hoare_vcg_imp_lift')
-  apply (wpsimp wp: update_sk_obj_ref_wp)
-  apply (wpsimp simp: has_budget_def2 wp: hoare_vcg_disj_lift)
-  apply (clarsimp simp: simple_obj_at_def valid_ntfn_q_def2 obj_at_def)
-   apply (case_tac "xa = ptr"; simp)
-   apply (drule_tac x=x and y = xa in spec2; clarsimp simp: has_budget_def2)
-   apply (drule_tac x=x and y = xa in spec2; clarsimp simp: has_budget_def2)
-  done
-
 lemma unbind_maybe_notification_valid_sched[wp]:
   "unbind_maybe_notification ptr \<lbrace>valid_sched_pred_strong P\<rbrace>"
   by (wpsimp wp: get_sk_obj_ref_wp simp: unbind_maybe_notification_def)
@@ -5038,10 +4929,13 @@ crunch simple[wp]: reply_remove simple_sched_action
   (simp: a_type_def wp: hoare_drop_imps)
 
 lemma sched_context_unbind_tcb_simple_sched_action[wp]:
-  "\<lbrace>simple_sched_action\<rbrace> sched_context_unbind_tcb sc_ptr \<lbrace>\<lambda>_. simple_sched_action\<rbrace>"
-  by (wpsimp simp: sched_context_unbind_tcb_def wp: get_sched_context_wp)
+  "sched_context_unbind_tcb sc_ptr \<lbrace>simple_sched_action\<rbrace>"
+  "sched_context_unbind_tcb sc_ptr \<lbrace>scheduler_act_sane\<rbrace>"
+  by (wpsimp simp: sched_context_unbind_tcb_def wp: get_sched_context_wp)+
 
-crunch simple[wp]: unbind_from_sc,sched_context_unbind_all_tcbs simple_sched_action
+crunches unbind_from_sc,sched_context_unbind_all_tcbs
+ for simple[wp]:  simple_sched_action
+ and scheduler_act_sane[wp]:  scheduler_act_sane
   (wp: maybeM_wp crunch_wps hoare_vcg_all_lift)
 
 crunch scheduler_act_not[wp]: unbind_from_sc "scheduler_act_not t"
@@ -5049,6 +4943,7 @@ crunch scheduler_act_not[wp]: unbind_from_sc "scheduler_act_not t"
 
 crunches cancel_ipc
 for simple_sched_action[wp]: simple_sched_action
+and scheduler_act_sane[wp]: scheduler_act_sane
 and scheduler_act_not[wp]: "scheduler_act_not t"
   (wp: maybeM_wp hoare_drop_imps)
 
@@ -5593,14 +5488,17 @@ lemma sched_context_unbind_tcb_valid_sched:
               simp: valid_sched_def)
   by (clarsimp simp: sc_at_pred_n_def obj_at_def)
 
+(* This precondition is nasty, but it's better than passing through sym_refs *)
 lemma maybe_sched_context_unbind_tcb_valid_sched:
-  "\<lbrace>valid_sched and scheduler_act_not tcb_ptr and (\<lambda>s. sym_refs (state_refs_of s))\<rbrace>
+  "\<lbrace>valid_sched and
+   (\<lambda>s. \<forall>scp tp. bound_sc_tcb_at (\<lambda>x. x = Some scp) tcb_ptr s \<longrightarrow>
+                 sc_tcb_sc_at (\<lambda>x. x = Some tp) scp s \<longrightarrow>
+                 scheduler_act_not tp s)\<rbrace>
    maybe_sched_context_unbind_tcb tcb_ptr
    \<lbrace>\<lambda>y. valid_sched\<rbrace>"
   unfolding maybe_sched_context_unbind_tcb_def
   apply (wpsimp wp: sched_context_unbind_tcb_valid_sched get_tcb_obj_ref_wp)
-  by (fastforce simp: sc_tcb_sc_at_def obj_at_def sym_refs_def state_refs_of_def get_refs_def2
-                split: option.splits)
+  by (clarsimp simp: pred_tcb_at_def obj_at_def sc_at_pred_n_def)
 
 lemma sched_context_unbind_all_tcbs_valid_sched[wp]:
   "\<lbrace>valid_sched and simple_sched_action\<rbrace>
@@ -5716,11 +5614,10 @@ lemma unbind_from_sc_valid_sched:
   unfolding unbind_from_sc_def
   by (wpsimp wp: hoare_drop_imps hoare_vcg_all_lift maybeM_wp sched_context_unbind_tcb_valid_sched)
 
-(* precondition could be weaker (invs > (sym_refs and valid_objs)) but
+(* precondition could be weaker (invs > (sym_refs and valid_objs and (\<lambda>s. cap \<noteq> ThreadCap idle_thread_ptr)) but
    this is much simpler to prove *)
 lemma finalise_cap_valid_sched[wp]:
-  "\<lbrace>valid_sched and invs and simple_sched_action and valid_cap cap and (\<lambda>s. \<exists>slot. cte_wp_at ((=) cap) slot s)
-    and (\<lambda>s. cap \<noteq> ThreadCap idle_thread_ptr)\<rbrace>
+  "\<lbrace>valid_sched and invs and simple_sched_action and (\<lambda>s. \<exists>slot. cte_wp_at ((=) cap) slot s)\<rbrace>
    finalise_cap cap final
    \<lbrace>\<lambda>_. valid_sched :: 'state_ext state \<Rightarrow> _\<rbrace>"
   supply if_split[split del]
@@ -5733,15 +5630,19 @@ lemma finalise_cap_valid_sched[wp]:
                  split: if_splits | strengthen invs_valid_idle invs_sym_refs)+)[1]
      apply ((wpsimp wp: cancel_ipc_valid_sched reply_remove_valid_sched gts_wp get_simple_ko_wp
                 split: if_splits| strengthen invs_valid_idle invs_sym_refs)+)[1]
-       apply (simp add: pred_tcb_at_eq_commute)
-      apply (clarsimp simp: tcb_at_kh_simps pred_map_def)
+     apply (simp add: pred_tcb_at_eq_commute)
+     apply (clarsimp simp: tcb_at_kh_simps pred_map_def)
     apply (wpsimp wp: suspend_valid_sched)
       apply (rule_tac Q="\<lambda>ya. valid_sched and invs and scheduler_act_not x7 and tcb_at x7"
                       in hoare_strengthen_post)
        apply (wpsimp wp: unbind_from_sc_valid_sched)
       apply fastforce
      apply (wpsimp wp: unbind_notification_invs split: if_splits)
-    apply (clarsimp simp: valid_cap_def split: if_splits)
+    apply (subgoal_tac "valid_cap cap s")
+     apply (clarsimp simp: valid_cap_def split: if_splits)
+     apply (frule(1) valid_global_refsD[OF invs_valid_global_refs _ idle_global])
+     apply (clarsimp dest!: invs_valid_idle simp: valid_idle_def cap_range_def)
+    apply (clarsimp elim!: cte_wp_valid_cap)
    apply (rename_tac scptr x)
    apply (wpsimp wp: set_sc_refill_max_valid_sched_unbound_sc hoare_vcg_all_lift)
     apply (rule_tac Q="\<lambda>ya. invs and sc_tcb_sc_at (\<lambda>x. x = None) scptr"
@@ -5756,43 +5657,48 @@ lemma finalise_cap_valid_sched[wp]:
   apply (wpsimp wp: deleting_irq_handler_valid_sched)
   done
 
-lemma store_word_offs_cur_sc_chargeable[wp]:
-  "store_word_offs a b c \<lbrace>cur_sc_chargeable\<rbrace>"
-  unfolding store_word_offs_def
-  by (wpsimp wp: set_object_wp)
-
-lemma set_mrs_cur_sc_chargeable[wp]:
-  "set_mrs thread buf msgs \<lbrace>cur_sc_chargeable\<rbrace>"
-  unfolding set_mrs_def
-  apply (wpsimp wp: set_object_wp zipWithM_x_inv')
-  by (clarsimp simp: cur_sc_chargeable_def bound_sc_tcb_at_kh_def obj_at_kh_def st_tcb_at_kh_def
-                 dest!: get_tcb_SomeD, fastforce)
-
 lemma cancel_all_ipc_simple_sched_action[wp]:
   "cancel_all_ipc ep \<lbrace>simple_sched_action :: 'state_ext state \<Rightarrow> _\<rbrace>"
-  by (wpsimp wp: get_simple_ko_wp simp: cancel_all_ipc_def)
+  "cancel_all_ipc ep \<lbrace>scheduler_act_sane :: 'state_ext state \<Rightarrow> _\<rbrace>"
+  by (wpsimp wp: get_simple_ko_wp simp: cancel_all_ipc_def)+
 
 lemma cancel_all_signals_simple_sched_action[wp]:
   "cancel_all_signals ntfn \<lbrace>simple_sched_action :: 'state_ext state \<Rightarrow> _\<rbrace>"
-  by (wpsimp wp: get_simple_ko_wp simp: cancel_all_signals_def)
+  "cancel_all_signals ntfn \<lbrace>scheduler_act_sane :: 'state_ext state \<Rightarrow> _\<rbrace>"
+  by (wpsimp wp: get_simple_ko_wp simp: cancel_all_signals_def)+
 
 lemma fast_finalise_simple_sched_action[wp]:
   "fast_finalise cap final \<lbrace>simple_sched_action :: 'state_ext state \<Rightarrow> _\<rbrace>"
-  by (cases cap; wpsimp wp: gts_wp get_simple_ko_wp)
+  "fast_finalise cap final \<lbrace>scheduler_act_sane :: 'state_ext state \<Rightarrow> _\<rbrace>"
+  by (cases cap; wpsimp wp: gts_wp get_simple_ko_wp)+
 
 lemma cap_delete_one_simple_sched_action[wp]:
   "cap_delete_one slot \<lbrace>simple_sched_action :: 'state_ext state \<Rightarrow> _\<rbrace>"
-  by (wpsimp wp: get_simple_ko_wp simp: cap_delete_one_def)
+  "cap_delete_one slot \<lbrace>scheduler_act_sane :: 'state_ext state \<Rightarrow> _\<rbrace>"
+  by (wpsimp wp: get_simple_ko_wp simp: cap_delete_one_def)+
 
 lemma deleting_irq_handler_simple_sched_action[wp]:
   "deleting_irq_handler irq \<lbrace>simple_sched_action :: 'state_ext state \<Rightarrow> _\<rbrace>"
-  by (wpsimp wp: get_simple_ko_wp simp: deleting_irq_handler_def)
+  "deleting_irq_handler irq \<lbrace>scheduler_act_sane :: 'state_ext state \<Rightarrow> _\<rbrace>"
+  by (wpsimp wp: get_simple_ko_wp simp: deleting_irq_handler_def)+
+
+crunches cancel_ipc, suspend, sched_context_unbind_all_tcbs
+  for scheduler_act_sane[wp]: "scheduler_act_sane :: 'state_ext state \<Rightarrow> _"
+  (wp: crunch_wps )
 
 lemma finalise_cap_simple_sched_action[wp]:
   "finalise_cap cap final \<lbrace>simple_sched_action :: 'state_ext state \<Rightarrow> _\<rbrace>"
-  by (cases cap; wpsimp wp: gts_wp get_simple_ko_wp)
+  "finalise_cap cap final \<lbrace>scheduler_act_sane :: 'state_ext state \<Rightarrow> _\<rbrace>"
+  by (cases cap; wpsimp wp: gts_wp get_simple_ko_wp)+
 
 end
+
+lemma update_time_stamp_valid_sched_misc[wp]:
+  "update_time_stamp \<lbrace>\<lambda>s. P (cur_sc s) (cur_domain s) (cur_thread s) (idle_thread s)
+          (ready_queues s) (release_queue s) (scheduler_action s)
+          (etcbs_of s) (tcb_sts_of s) (tcb_scps_of s) (sc_refill_cfgs_of s)\<rbrace>"
+  unfolding update_time_stamp_def
+  by wpsimp
 
 context DetSchedSchedule_AI_det_ext begin
 
@@ -5812,9 +5718,6 @@ lemma rec_del_valid_sched:
     apply (rule use_spec)
     apply (rule rec_del_invs''[where Q="valid_sched and simple_sched_action"])
          apply wpsimp+
-       apply (clarsimp simp: invs_valid_objs cte_wp_valid_cap)
-       apply (frule(1) valid_global_refsD[OF invs_valid_global_refs _ idle_global])
-       apply (clarsimp dest!: invs_valid_idle simp: valid_idle_def cap_range_def)
       apply (wpsimp wp: preemption_point_inv')+
   done
 
@@ -5822,209 +5725,110 @@ lemma rec_del_simple_sched_action[wp]:
   "\<lbrace>simple_sched_action\<rbrace> rec_del call \<lbrace>\<lambda>rv. simple_sched_action :: det_state \<Rightarrow> _\<rbrace>"
    by (wpsimp wp: rec_del_preservation preemption_point_inv' finalise_cap_simple_sched_action)
 
-lemma arch_post_cap_deletion_scheduler_act_sane[wp]:
-  "arch_post_cap_deletion x \<lbrace>scheduler_act_sane :: det_state \<Rightarrow> _\<rbrace>"
-  apply (rule hoare_weaken_pre)
-  apply (wps ARM.arch_post_cap_deletion_cur_thread)
-  apply wpsimp+
-  done
-
-crunch scheduler_act_sane[wp]: cap_swap_for_delete, empty_slot "scheduler_act_sane :: det_state \<Rightarrow> _"
-  (simp: unless_def wp: maybeM_inv ignore: set_object)
+end
 
 lemma possible_switch_to_scheduler_act_sane:
   "\<lbrace>scheduler_act_sane and (\<lambda>s. scheduler_action s = resume_cur_thread \<longrightarrow> not_in_release_q t s \<longrightarrow> t \<noteq> cur_thread s)\<rbrace>
    possible_switch_to t
-   \<lbrace>\<lambda>_. scheduler_act_sane :: det_state \<Rightarrow> _\<rbrace>"
+   \<lbrace>\<lambda>_. scheduler_act_sane\<rbrace>"
   unfolding possible_switch_to_def
-  apply (wpsimp wp: set_scheduler_action_wp get_tcb_obj_ref_wp)
-  by (clarsimp simp: scheduler_act_sane_def)
+  apply (wpsimp wp: set_scheduler_action_wp get_tcb_obj_ref_wp thread_get_wp)
+  by (clarsimp simp: scheduler_act_sane_def obj_at_def is_tcb)
+
+(* FIXME: add this to elim set much higher up *)
+declare pred_tcb_at_tcb_at[elim!]
 
 lemma possible_switch_to_scheduler_act_sane':
   "\<lbrace>scheduler_act_sane and (\<lambda>s. t \<noteq> cur_thread s)\<rbrace>
    possible_switch_to t
-   \<lbrace>\<lambda>_. scheduler_act_sane :: det_state \<Rightarrow> _\<rbrace>"
+   \<lbrace>\<lambda>_. scheduler_act_sane\<rbrace>"
   unfolding possible_switch_to_def
-  apply (wpsimp wp: set_scheduler_action_wp get_tcb_obj_ref_wp)
-  by (clarsimp simp: scheduler_act_sane_def)
+  apply (wpsimp wp: set_scheduler_action_wp get_tcb_obj_ref_wp thread_get_wp)
+  by (clarsimp simp: scheduler_act_sane_def obj_at_def is_tcb)
 
 lemma restart_thread_if_no_fault_scheduler_act_sane[wp]:
- "\<lbrace>scheduler_act_sane and (\<lambda>s. xa \<noteq> cur_thread s) and tcb_at xa\<rbrace>
+ "\<lbrace>scheduler_act_sane and (\<lambda>s. xa \<noteq> cur_thread s) \<rbrace>
   restart_thread_if_no_fault xa
-  \<lbrace>\<lambda>_. scheduler_act_sane:: det_state \<Rightarrow> _\<rbrace>"
+  \<lbrace>\<lambda>_. scheduler_act_sane\<rbrace>"
   unfolding restart_thread_if_no_fault_def
-  by (wpsimp simp: set_thread_state_def set_thread_state_act_def
+  by (wpsimp simp: set_thread_state_def set_thread_state_act_def thread_get_def
                wp: possible_switch_to_scheduler_act_sane set_scheduler_action_wp is_schedulable_wp
-                   set_object_wp thread_get_wp
+                   set_object_wp
                    hoare_vcg_imp_lift' )
 
 lemma tcb_sched_enqueue_ct_not_queued:
   "\<lbrace> ct_not_queued and (\<lambda>s. cur \<noteq> cur_thread s)\<rbrace>
    tcb_sched_action tcb_sched_enqueue cur
    \<lbrace>\<lambda>_. ct_not_queued\<rbrace>"
-  apply (wpsimp simp: tcb_sched_action_def thread_get_def)
-  by (fastforce simp: not_queued_def tcb_sched_enqueue_def)
+  apply (wpsimp simp: tcb_sched_action_def thread_get_def wp: set_tcb_queue_wp get_tcb_queue_wp)
+  by (clarsimp simp: in_queues_2_def tcb_sched_ready_q_update_set_simps)
 
 lemma possible_switch_to_ct_not_queued:
   "\<lbrace>ct_not_queued and (\<lambda>s. t \<noteq> cur_thread s) and scheduler_act_sane\<rbrace> possible_switch_to t \<lbrace>\<lambda>_. ct_not_queued\<rbrace>"
   apply (simp add: possible_switch_to_def)
   apply (rule hoare_seq_ext[OF _ gsc_sp])
-  apply (wpsimp wp: tcb_sched_enqueue_ct_not_queued)
+  apply (wpsimp wp: tcb_sched_enqueue_ct_not_queued thread_get_wp)
   done
 
 lemma restart_thread_if_no_fault_ct_not_queued[wp]:
- "\<lbrace>ct_not_queued and scheduler_act_sane and (\<lambda>s. xa \<noteq> cur_thread s) and tcb_at xa\<rbrace>
+ "\<lbrace>ct_not_queued and scheduler_act_sane and (\<lambda>s. xa \<noteq> cur_thread s)\<rbrace>
   restart_thread_if_no_fault xa
-  \<lbrace>\<lambda>_. ct_not_queued:: det_state \<Rightarrow> _\<rbrace>"
+  \<lbrace>\<lambda>_. ct_not_queued\<rbrace>"
   unfolding restart_thread_if_no_fault_def
-  by (wpsimp simp: set_thread_state_def set_thread_state_act_def
+  by (wpsimp simp: set_thread_state_def set_thread_state_act_def thread_get_def
                wp: possible_switch_to_ct_not_queued set_scheduler_action_wp is_schedulable_wp
-                   set_object_wp thread_get_wp
+                   set_object_wp
                    hoare_vcg_imp_lift' )
 
 crunches cancel_all_ipc
-  for ct_not_in_release_q[wp]: "ct_not_in_release_q :: det_state \<Rightarrow> _"
+  for ct_not_in_release_q[wp]: "ct_not_in_release_q"
   (wp: crunch_wps)
 
-lemma cancel_all_ipc_scheduler_act_sane[wp]:
- "\<lbrace>scheduler_act_sane and valid_ep_q:: det_state \<Rightarrow> _\<rbrace>
-  cancel_all_ipc epptr
-  \<lbrace>\<lambda>_. scheduler_act_sane\<rbrace>"
-  unfolding cancel_all_ipc_def
-  apply (rule hoare_seq_ext[OF _ get_simple_ko_sp])
-  apply (case_tac "ep=IdleEP"; simp?)
-   apply wpsimp
-  apply wpc
-     apply wpsimp
-    apply (rule_tac Q="\<lambda>s. (ko_at (Endpoint ep) epptr and scheduler_act_sane and valid_ep_q) s" in hoare_weaken_pre)
-     apply (rule hoare_seq_ext[OF _ get_epq_sp])
-     apply wpsimp
-       apply (rule_tac Q="\<lambda>_. scheduler_act_sane and (\<lambda>x. \<forall>t. t \<in> set (queue) \<longrightarrow> tcb_at t x \<and> t \<noteq> cur_thread x)" in hoare_strengthen_post)
-        apply (wpsimp wp: mapM_x_wp hoare_vcg_all_lift hoare_vcg_imp_lift' gts_wp)
-         prefer 2
-         apply (rule subset_refl, clarsimp, clarsimp)
-      apply (wpsimp wp: hoare_vcg_all_lift hoare_vcg_imp_lift')
-     apply (clarsimp simp: valid_ep_q_def obj_at_def)
-     apply (drule_tac x=epptr in spec)
-     apply clarsimp
-     apply (drule_tac x=x in bspec, simp)
-     apply (clarsimp simp: pred_tcb_at_def obj_at_def is_tcb)
-    apply assumption
-   apply (rule_tac Q="\<lambda>s. (ko_at (Endpoint ep) epptr and scheduler_act_sane and valid_ep_q) s" in hoare_weaken_pre)
-    apply (rule hoare_seq_ext[OF _ get_epq_sp])
-    apply wpsimp
-      apply (rule_tac Q="\<lambda>_. scheduler_act_sane and (\<lambda>x. \<forall>t. t \<in> set (queue) \<longrightarrow> tcb_at t x \<and> t \<noteq> cur_thread x)" in hoare_strengthen_post)
-       apply (wpsimp wp: mapM_x_wp hoare_vcg_all_lift hoare_vcg_imp_lift' gts_wp)
-        prefer 2
-        apply (rule subset_refl, clarsimp, clarsimp)
-     apply (wpsimp wp: hoare_vcg_all_lift hoare_vcg_imp_lift')
-    apply (clarsimp simp: valid_ep_q_def obj_at_def)
-    apply (drule_tac x=epptr in spec)
-    apply clarsimp
-    apply (drule_tac x=x in bspec, simp)
-    apply (clarsimp simp: pred_tcb_at_def obj_at_def is_tcb)
-   apply assumption
-  apply fastforce
-  done
-
-
 crunches update_time_stamp
-  for release_queue[wp]: "\<lambda>s. P (release_queue s)"
-  and ready_queues[wp]: "\<lambda>s. P (ready_queues s)"
-  and cur_sc[wp]: "\<lambda>s. P (cur_sc s)"
-
-lemma update_time_stamp_is_refill_sufficient[wp]:
-  "update_time_stamp \<lbrace>is_refill_sufficient scp k\<rbrace>"
-  unfolding update_time_stamp_def
-  apply (wpsimp simp: do_machine_op_def)
-  apply (clarsimp simp: budget_sufficient_defs sc_at_pred_n_def  split: option.splits)
-  done
-
-crunches update_time_stamp
-  for ready_queues[wp]: "\<lambda>s. P (ready_queues s)"
-  and cur_domain[wp]: "\<lambda>s. P (cur_domain s)"
-  and idle_thread[wp]: "\<lambda>s. P (idle_thread s)"
-  and release_queue[wp]: "\<lambda>s. P (release_queue s)"
-  and typ_at[wp]: "\<lambda>s. P (typ_at T t  s)"
-  and etcbs_of[wp]: "\<lambda>s. P (etcbs_of s)"
-  and cur_sc[wp]: "\<lambda>s. P (cur_sc s)"
+  for typ_at[wp]: "\<lambda>s. P (typ_at T t  s)"
   and sc_at_pred_n[wp]: "\<lambda>s. Q (sc_at_pred_n N p P t s)"
 
-lemma tcb_ready_time_cur_time_update:
-  "P (tcb_ready_time t (s\<lparr>cur_time := new\<rparr>)) = P (tcb_ready_time t s)"
-  by (clarsimp simp: tcb_ready_time_def get_tcb_def dest!: get_tcb_SomeD split: option.splits)
-
 crunches update_time_stamp
-  for tcb_ready_time[wp]: "\<lambda>s. P (tcb_ready_time t s)"
-  (wp: crunch_wps simp: crunch_simps tcb_ready_time_cur_time_update)
+  for obj_at[wp]: "\<lambda>(s). Q (obj_at P t s)"
 
-lemma update_time_stamp_ct_not_in_queues[wp]:
- "update_time_stamp \<lbrace>ct_not_in_release_q\<rbrace>"
- "update_time_stamp \<lbrace>ct_not_queued\<rbrace>"
-  unfolding update_time_stamp_def
-  by (wpsimp simp: | wps)+
-
-lemma update_time_stamp_active_sc_tcb_at[wp]:
- "update_time_stamp \<lbrace>\<lambda>s. P (active_sc_tcb_at t s)\<rbrace>"
-  apply (rule bool_to_bool_cases[of P]; wpsimp)
-   apply (rule_tac Q="\<lambda>_ s. \<exists>scp. bound_sc_tcb_at (\<lambda>ko. ko = Some scp) t s \<and> sc_at_pred sc_refill_max (\<lambda>x. 0 < x ) scp s"
-    in hoare_strengthen_post)
-    apply (wpsimp wp: hoare_vcg_ex_lift hoare_vcg_imp_lift)
-    apply (clarsimp simp: active_sc_tcb_at_defs sc_at_pred_n_def split: option.splits)
-    apply (case_tac y; simp)
-   apply (fastforce simp: active_sc_tcb_at_defs sc_at_pred_n_def split: option.splits)
-  apply (rule_tac Q="\<lambda>_ s. \<forall>scp. ~ bound_sc_tcb_at (\<lambda>ko. ko = Some scp) t s \<or> ~sc_at_pred sc_refill_max (\<lambda>x. 0 < x ) scp s"
-   in hoare_strengthen_post)
-   apply (wpsimp wp: hoare_vcg_all_lift hoare_vcg_imp_lift)
-   apply (clarsimp simp: active_sc_tcb_at_defs sc_at_pred_n_def split: option.splits)
-  apply (clarsimp simp: active_sc_tcb_at_defs sc_at_pred_n_def split: option.splits)
-  apply (case_tac x2; simp)
-  done
-
-lemma update_time_stamp_budget_sufficient[wp]:
- "update_time_stamp \<lbrace>budget_sufficient t\<rbrace>"
-  apply (rule_tac Q="\<lambda>_ s. \<exists>scp. bound_sc_tcb_at (\<lambda>ko. ko = Some scp) t s \<and> sc_at_pred sc_refills (\<lambda>x. sufficient_refills 0 x ) scp s"
-   in hoare_strengthen_post)
-   apply (wpsimp wp: hoare_vcg_ex_lift hoare_vcg_imp_lift)
-   apply (clarsimp simp: budget_sufficient_defs sc_at_pred_n_def split: option.splits)
-  apply (clarsimp simp: budget_sufficient_defs sc_at_pred_n_def split: option.splits)
-  done
-
-lemma update_time_stamp_bound_cur_sc_tcb[wp]:
-  "update_time_stamp \<lbrace>\<lambda>s. bound_sc_tcb_at (\<lambda>x. x = Some (cur_sc s)) (cur_thread s) s\<rbrace>"
-  apply (rule hoare_lift_Pf[where f=cur_thread])
-  apply (rule hoare_lift_Pf[where f=cur_sc])
-  by wpsimp+
-
-lemma update_time_stamp_cur_sc_chargeable[wp]:
-  "update_time_stamp \<lbrace>cur_sc_chargeable\<rbrace>"
-  by (wpsimp simp: cur_sc_chargeable_def2 wp: hoare_vcg_imp_lift hoare_vcg_all_lift | wps)+
-
-crunches update_time_stamp
-  for obj_at[wp]: "\<lambda>(s::det_state). Q (obj_at P t s)"
+context DetSchedSchedule_AI begin
 
 lemma dmo_getCurrentTime_sp[wp]:
   "do_machine_op getCurrentTime \<lbrace>P\<rbrace> \<Longrightarrow>
-   \<lbrace>valid_machine_time and P :: det_state \<Rightarrow> _\<rbrace>
+   \<lbrace>valid_machine_time and P :: 'state_ext state \<Rightarrow> _\<rbrace>
    do_machine_op getCurrentTime
-   \<lbrace>\<lambda>rv s. (cur_time s \<le> rv) \<and> (rv \<le> - kernelWCET_ticks - 1) \<and>  P s\<rbrace>"
+   \<lbrace>\<lambda>rv s. (cur_time s \<le> rv) \<and> (rv \<le> - kernelWCET_ticks - 1) \<and> P s\<rbrace>"
   apply (rule_tac Q="\<lambda>rv s. P s \<and> ((cur_time s \<le> rv) \<and> (rv \<le> - kernelWCET_ticks - 1))" in hoare_strengthen_post)
   apply (wp hoare_vcg_conj_lift)
   apply (rule dmo_getCurrentTime_vmt_sp)
   by simp+
 
+(* This is not strictly a weakest precondition rule, but it is quite close. *)
+lemma dmo_getCurrentTime_wp:
+  assumes str_post: "(\<forall>rv s. (cur_time s \<le> rv) \<and> (rv \<le> - kernelWCET_ticks - 1) \<and> P s \<longrightarrow> Q rv s)"
+  assumes dmo_inv: "do_machine_op getCurrentTime \<lbrace>P\<rbrace>"
+  shows "\<lbrace>valid_machine_time and P :: 'state_ext state \<Rightarrow> _\<rbrace>
+         do_machine_op getCurrentTime
+         \<lbrace>\<lambda>rv s. Q rv s\<rbrace>"
+  apply (rule_tac Q="\<lambda>rv s. P s \<and> ((cur_time s \<le> rv) \<and> (rv \<le> - kernelWCET_ticks - 1))" in hoare_strengthen_post)
+  apply (wp hoare_vcg_conj_lift)
+  apply (rule dmo_inv)
+  apply (rule dmo_getCurrentTime_vmt_sp)
+  apply simp
+  using str_post apply_trace (fastforce)
+  done
+
 lemma update_time_stamp_is_refill_ready[wp]:
- "\<lbrace>valid_machine_time and is_refill_ready scp 0 :: det_state \<Rightarrow> _\<rbrace>
+ "\<lbrace>valid_machine_time and is_refill_ready scp :: 'state_ext state \<Rightarrow> _\<rbrace>
   update_time_stamp
-  \<lbrace>\<lambda>_. is_refill_ready scp 0\<rbrace>"
+  \<lbrace>\<lambda>_. is_refill_ready scp\<rbrace>"
   unfolding update_time_stamp_def
-  apply (rule_tac hoare_seq_ext[OF _ gets_sp])
-  apply (rule_tac Q="valid_machine_time and (is_refill_ready scp 0 and
-                     (\<lambda>s. cur_time s = prev_time))" in hoare_weaken_pre[rotated])
-   apply clarsimp
-  apply (rule_tac hoare_seq_ext[OF _ dmo_getCurrentTime_sp])
+  apply (wpsimp wp: dmo_getCurrentTime_wp)
+  prefer 2
+  apply (rule_tac Q="(is_refill_ready scp and
+                     (\<lambda>s. cur_time s = prev_time))" in hoare_weaken_pre[rotated], assumption)
    apply (wpsimp simp: )
-   apply (clarsimp simp: is_refill_ready_def obj_at_def)
+   apply (clarsimp simp: vs_all_heap_simps refills_ready_def)
    apply (rule_tac b="cur_time s + kernelWCET_ticks" in order.trans, simp)
    apply (rule word_plus_mono_left, simp)
    apply (subst olen_add_eqv)
@@ -6034,71 +5838,26 @@ lemma update_time_stamp_is_refill_ready[wp]:
    using kernelWCET_ticks_non_zero
    apply fastforce
   apply wpsimp
-  done
+  by simp
 
 lemma update_time_stamp_budget_ready[wp]:
- "\<lbrace>budget_ready t and valid_machine_time :: det_state \<Rightarrow> _\<rbrace>
+ "\<lbrace>budget_ready t and valid_machine_time :: 'state_ext state \<Rightarrow> _\<rbrace>
   update_time_stamp
   \<lbrace>\<lambda>_. budget_ready t\<rbrace>"
   apply (rule_tac Q="\<lambda>_ s. \<exists>scp. bound_sc_tcb_at (\<lambda>ko. ko = Some scp) t s \<and>
-                                 is_refill_ready scp 0 s"
+                                 is_refill_ready scp s"
    in hoare_strengthen_post)
    apply (wpsimp wp: hoare_vcg_ex_lift hoare_vcg_imp_lift)
-   apply (clarsimp simp: budget_ready_defs sc_at_pred_n_def split: option.splits)
-  apply (clarsimp simp: budget_sufficient_defs sc_at_pred_n_def split: option.splits)
+   apply (clarsimp simp: vs_all_heap_simps tcb_at_kh_simps)
+  apply (clarsimp simp: vs_all_heap_simps tcb_at_kh_simps)
   done
 
-lemma update_time_stamp_valid_ipc_queues[wp]:
-  "\<lbrace>valid_ep_q and valid_machine_time\<rbrace>
-   update_time_stamp
-   \<lbrace>\<lambda>_. valid_ep_q ::det_state \<Rightarrow> _\<rbrace>"
-  "\<lbrace>valid_ntfn_q and valid_machine_time\<rbrace>
-   update_time_stamp
-   \<lbrace>\<lambda>_. valid_ntfn_q ::det_state \<Rightarrow> _\<rbrace>"
-  by (wpsimp wp: valid_ntfn_q_lift_pre_conj[where R=valid_machine_time]
-                 valid_ep_q_lift_pre_conj[where R=valid_machine_time]
-                 hoare_vcg_disj_lift)+
+end
 
-lemma cancel_all_signals_scheduler_act_sane[wp]:
- "\<lbrace>scheduler_act_sane and valid_ntfn_q:: det_state \<Rightarrow> _\<rbrace>
-  cancel_all_signals f
-  \<lbrace>\<lambda>_. scheduler_act_sane\<rbrace>"
-  unfolding cancel_all_signals_def
-  apply (rule hoare_seq_ext[OF _ get_simple_ko_sp])
-  apply wpc
-     apply wpsimp
-    apply (rule_tac Q="\<lambda>s. (ko_at (Notification ntfn) f and scheduler_act_sane and valid_ntfn_q) s" in hoare_weaken_pre[rotated])
-     apply assumption
-    apply wpsimp
-      apply (rule_tac Q="\<lambda>_. scheduler_act_sane and (\<lambda>s. \<forall>x \<in> set x2. x \<noteq> (cur_thread s))" in hoare_strengthen_post)
-       apply (wpsimp wp: mapM_x_wp[where xs = t and S = "set t" for t, simplified])
-        apply (wpsimp wp: possible_switch_to_scheduler_act_sane')+
-       apply fastforce
-      apply fastforce
-     apply (wpsimp wp: )+
-    apply (clarsimp simp: valid_ntfn_q_def obj_at_def)
-    apply (drule_tac x=f in spec, fastforce simp: ntfn_queue_def)
-   apply wpsimp
-  apply clarsimp
-  done
-
-crunches unbind_maybe_notification, sched_context_maybe_unbind_ntfn, cancel_ipc, suspend
-  for scheduler_act_sane[wp]: "scheduler_act_sane :: det_state \<Rightarrow> _"
-  (wp: crunch_wps)
-
-lemma misc_arch_scheduler_act_sane[wp]:
-  "prepare_thread_delete x \<lbrace>scheduler_act_sane :: det_state \<Rightarrow> _\<rbrace>"
-  "arch_finalise_cap z b \<lbrace>scheduler_act_sane :: det_state \<Rightarrow> _\<rbrace>"
-  by (rule hoare_weaken_pre, wps | wpsimp)+
-
-crunches complete_yield_to, sched_context_unbind_tcb, unbind_from_sc, unbind_notification,
-         sched_context_unbind_yield_from, sched_context_unbind_reply, sched_context_unbind_ntfn,
-         sched_context_unbind_all_tcbs
-  for scheduler_act_sane[wp]: "scheduler_act_sane :: det_state \<Rightarrow> _"
-  (wp: crunch_wps maybeM_inv)
+context DetSchedSchedule_AI_det_ext begin
 
 lemma fast_finalise_scheduler_act_sane[wp]:
-  "\<lbrace>scheduler_act_sane and valid_ep_q and valid_ntfn_q\<rbrace>
+  "\<lbrace>scheduler_act_sane and schedulable_ipc_queues and ct_not_blocked\<rbrace>
    fast_finalise cap x
    \<lbrace>\<lambda>_. scheduler_act_sane :: det_state \<Rightarrow> _\<rbrace>"
   apply (case_tac cap)
@@ -6106,22 +5865,54 @@ lemma fast_finalise_scheduler_act_sane[wp]:
   done
 
 lemma deleting_irq_handler_scheduler_act_sane[wp]:
-  "\<lbrace>scheduler_act_sane and valid_ep_q and valid_ntfn_q\<rbrace>
+  "\<lbrace>scheduler_act_sane and schedulable_ipc_queues and ct_not_blocked\<rbrace>
    deleting_irq_handler y
    \<lbrace>\<lambda>_. scheduler_act_sane :: det_state \<Rightarrow> _\<rbrace>"
   unfolding deleting_irq_handler_def
   by (wpsimp simp: cap_delete_one_def wp: hoare_drop_imp hoare_vcg_if_lift2)
 
-lemma finalise_cap_scheduler_act_sane[wp]:
-  "\<lbrace>scheduler_act_sane and valid_ep_q and valid_ntfn_q\<rbrace>
-   finalise_cap cap param_b
-   \<lbrace>\<lambda>_. scheduler_act_sane:: det_state \<Rightarrow> _\<rbrace>"
-  apply (case_tac cap)
-               apply ((wpsimp wp: gts_wp get_simple_ko_wp | intro conjI impI)+)
+
+lemma sym_refs_SendEP_ipc_queued_thread:
+  "\<lbrakk> kheap s ptr = Some (Endpoint (SendEP q)); sym_refs (state_refs_of s); t \<in> set q \<rbrakk>
+   \<Longrightarrow> ipc_queued_thread t s"
+  apply (clarsimp simp: sym_refs_def)
+  apply (erule_tac x = ptr in allE)
+  apply (drule_tac x = "(t, EPSend)" in bspec)
+   apply (clarsimp simp: state_refs_of_def)
+  apply (clarsimp simp: state_refs_of_def refs_of_def split: option.splits)
+  apply (case_tac x2;
+         clarsimp simp: get_refs_def tcb_st_refs_of_def vs_all_heap_simps
+                 split: option.splits thread_state.splits)
   done
 
-lemma cancel_all_ipc_ct_not_queued[wp]:
-  "\<lbrace>ct_not_queued and scheduler_act_sane and valid_ep_q\<rbrace>
+lemma sym_refs_RecvEP_ipc_queued_thread:
+  "\<lbrakk> kheap s ptr = Some (Endpoint (RecvEP q)); sym_refs (state_refs_of s); t \<in> set q \<rbrakk>
+   \<Longrightarrow> ipc_queued_thread t s"
+  apply (clarsimp simp: sym_refs_def)
+  apply (erule_tac x = ptr in allE)
+  apply (drule_tac x = "(t, EPRecv)" in bspec)
+   apply (clarsimp simp: state_refs_of_def)
+  apply (clarsimp simp: state_refs_of_def refs_of_def split: option.splits)
+  apply (case_tac x2;
+         clarsimp simp: get_refs_def tcb_st_refs_of_def vs_all_heap_simps
+                 split: option.splits thread_state.splits)
+  done
+
+lemma sym_refs_WaitingNtfn_ipc_queued_thread:
+  "\<lbrakk> kheap s ptr = Some (Notification (ntfn)); ntfn_obj ntfn = WaitingNtfn q;  sym_refs (state_refs_of s); t \<in> set q \<rbrakk>
+   \<Longrightarrow> ipc_queued_thread t s"
+  apply (clarsimp simp: sym_refs_def)
+  apply (erule_tac x = ptr in allE)
+  apply (drule_tac x = "(t, NTFNSignal)" in bspec)
+   apply (clarsimp simp: state_refs_of_def ntfn_q_refs_of_def)
+  apply (clarsimp simp: state_refs_of_def refs_of_def split: option.splits)
+  apply (case_tac x2;
+         clarsimp simp: get_refs_def tcb_st_refs_of_def vs_all_heap_simps
+                 split: option.splits thread_state.splits)
+  done
+
+lemma cancel_all_ipc_ct_not_queued:
+  "\<lbrace>ct_not_queued and scheduler_act_sane and invs and ct_not_blocked\<rbrace>
    cancel_all_ipc epptr
    \<lbrace>\<lambda>_. ct_not_queued:: det_state \<Rightarrow> _\<rbrace>"
   unfolding cancel_all_ipc_def
@@ -6130,46 +5921,44 @@ lemma cancel_all_ipc_ct_not_queued[wp]:
    apply wpsimp
   apply wpc
      apply wpsimp
-    apply (rule_tac Q="\<lambda>s. (ko_at (Endpoint ep) epptr and ct_not_queued and scheduler_act_sane and valid_ep_q) s" in hoare_weaken_pre)
+    apply (rule_tac Q="\<lambda>s. (ko_at (Endpoint ep) epptr and ct_not_queued and scheduler_act_sane and invs and ct_not_blocked) s" in hoare_weaken_pre)
      apply (rule hoare_seq_ext[OF _ get_epq_sp])
      apply wpsimp
-       apply (rule_tac Q="\<lambda>_. ct_not_queued and scheduler_act_sane and (\<lambda>x. \<forall>t. t \<in> set (queue) \<longrightarrow> tcb_at t x \<and> t \<noteq> cur_thread x)" in hoare_strengthen_post)
-        apply (wpsimp wp: mapM_x_wp hoare_vcg_all_lift hoare_vcg_imp_lift' gts_wp)
+       apply (rule_tac Q="\<lambda>_. ct_not_queued and scheduler_act_sane and (\<lambda>x. \<forall>t. t \<in> set (queue) \<longrightarrow> t \<noteq> cur_thread x)" in hoare_strengthen_post)
+        apply_trace (wpsimp wp: mapM_x_wp hoare_vcg_all_lift hoare_vcg_imp_lift' gts_wp)
          prefer 2
          apply (rule subset_refl, clarsimp, clarsimp)
       apply (wpsimp wp: hoare_vcg_all_lift hoare_vcg_imp_lift')
-     apply (clarsimp simp: valid_ep_q_def obj_at_def)
-     apply (drule_tac x=epptr in spec)
-     apply clarsimp
-     apply (drule_tac x=x in bspec, simp)
-     apply (clarsimp simp: pred_tcb_at_def obj_at_def is_tcb)
+     apply (clarsimp simp: obj_at_def)
+     apply (subgoal_tac "ipc_queued_thread (cur_thread s) s")
+      apply (clarsimp simp: ct_in_state_def tcb_at_kh_simps pred_map_simps)
+     apply (erule sym_refs_SendEP_ipc_queued_thread; clarsimp)
     apply assumption
-   apply (rule_tac Q="\<lambda>s. (ko_at (Endpoint ep) epptr and ct_not_queued and scheduler_act_sane and valid_ep_q) s" in hoare_weaken_pre)
+   apply (rule_tac Q="\<lambda>s. (ko_at (Endpoint ep) epptr and ct_not_queued and scheduler_act_sane and invs and ct_not_blocked) s" in hoare_weaken_pre)
     apply (rule hoare_seq_ext[OF _ get_epq_sp])
     apply wpsimp
-      apply (rule_tac Q="\<lambda>_. ct_not_queued and scheduler_act_sane and (\<lambda>x. \<forall>t. t \<in> set (queue) \<longrightarrow> tcb_at t x \<and> t \<noteq> cur_thread x)" in hoare_strengthen_post)
+      apply (rule_tac Q="\<lambda>_. ct_not_queued and scheduler_act_sane and (\<lambda>x. \<forall>t. t \<in> set (queue) \<longrightarrow> t \<noteq> cur_thread x)" in hoare_strengthen_post)
        apply (wpsimp wp: mapM_x_wp hoare_vcg_all_lift hoare_vcg_imp_lift' gts_wp)
         prefer 2
         apply (rule subset_refl, clarsimp, clarsimp)
      apply (wpsimp wp: hoare_vcg_all_lift hoare_vcg_imp_lift')
-    apply (clarsimp simp: valid_ep_q_def obj_at_def)
-    apply (drule_tac x=epptr in spec)
-    apply clarsimp
-    apply (drule_tac x=x in bspec, simp)
-    apply (clarsimp simp: pred_tcb_at_def obj_at_def is_tcb)
+    apply (clarsimp simp: obj_at_def)
+    apply (subgoal_tac "ipc_queued_thread (cur_thread s) s")
+     apply (clarsimp simp: ct_in_state_def tcb_at_kh_simps pred_map_simps)
+    apply (erule sym_refs_RecvEP_ipc_queued_thread; clarsimp)
    apply assumption
   apply fastforce
   done
 
-lemma cancel_all_signals_ct_not_queued[wp]:
- "\<lbrace>ct_not_queued and scheduler_act_sane and valid_ntfn_q:: det_state \<Rightarrow> _\<rbrace>
+lemma cancel_all_signals_ct_not_queued:
+ "\<lbrace>ct_not_queued and scheduler_act_sane and invs and ct_not_blocked:: det_state \<Rightarrow> _\<rbrace>
   cancel_all_signals f
   \<lbrace>\<lambda>_. ct_not_queued\<rbrace>"
   unfolding cancel_all_signals_def
   apply (rule hoare_seq_ext[OF _ get_simple_ko_sp])
   apply wpc
      apply wpsimp
-    apply (rule_tac Q="\<lambda>s. (ko_at (Notification ntfn) f and ct_not_queued and scheduler_act_sane and valid_ntfn_q) s" in hoare_weaken_pre[rotated])
+    apply (rule_tac Q="\<lambda>s. (ko_at (Notification ntfn) f and ct_not_queued and scheduler_act_sane and invs and ct_not_blocked) s" in hoare_weaken_pre[rotated])
      apply assumption
     apply wpsimp
       apply (rule_tac Q="\<lambda>_. ct_not_queued and scheduler_act_sane and (\<lambda>s. \<forall>x \<in> set x2. x \<noteq> (cur_thread s))" in hoare_strengthen_post)
@@ -6178,8 +5967,10 @@ lemma cancel_all_signals_ct_not_queued[wp]:
        apply fastforce
       apply fastforce
      apply (wpsimp wp: )+
-    apply (clarsimp simp: valid_ntfn_q_def obj_at_def)[1]
-    apply (drule_tac x=f in spec, fastforce simp: ntfn_queue_def)
+    apply (clarsimp simp: obj_at_def)
+    apply (subgoal_tac "ipc_queued_thread (cur_thread s) s")
+     apply (clarsimp simp: ct_in_state_def tcb_at_kh_simps pred_map_simps)
+    apply (erule (1) sym_refs_WaitingNtfn_ipc_queued_thread; clarsimp)
    apply wpsimp
   apply clarsimp
   done
@@ -6198,32 +5989,9 @@ crunches reply_remove, suspend, complete_yield_to, sched_context_unbind_tcb, unb
   for ct_not_queued[wp]: "ct_not_queued :: det_state \<Rightarrow> _"
   (wp: crunch_wps maybeM_wp tcb_sched_dequeue_ct_not_queued simp: crunch_simps ignore: tcb_sched_action)
 
-lemma misc_arch_ct_queue_lemmas[wp]:
-  "arch_post_cap_deletion x \<lbrace>ct_not_in_release_q :: det_state \<Rightarrow> _\<rbrace>"
-  "prepare_thread_delete x2 \<lbrace>ct_not_in_release_q :: det_state \<Rightarrow> _\<rbrace>"
-  "arch_finalise_cap a b \<lbrace>ct_not_in_release_q :: det_state \<Rightarrow> _\<rbrace> "
-  "arch_post_cap_deletion x \<lbrace>ct_not_queued :: det_state \<Rightarrow> _\<rbrace>"
-  "prepare_thread_delete x2 \<lbrace>ct_not_queued :: det_state \<Rightarrow> _\<rbrace>"
-  "arch_finalise_cap a b \<lbrace>ct_not_queued :: det_state \<Rightarrow> _\<rbrace> "
-  apply (rule hoare_weaken_pre, wps, wpsimp, simp)+
-  done
-
-crunches empty_slot
-  for ct_not_queued[wp]: "ct_not_queued :: det_state \<Rightarrow> _"
+crunches deleting_irq_handler
+  for ct_not_in_release_q[wp]: "ct_not_in_release_q :: det_state \<Rightarrow> _"
   (wp: crunch_wps)
-
-lemma fast_finalise_ct_not_queued[wp]:
-  "\<lbrace>ct_not_queued and scheduler_act_sane and valid_ntfn_q and valid_ep_q\<rbrace> fast_finalise cap x \<lbrace>\<lambda>_. ct_not_queued :: det_state \<Rightarrow> _\<rbrace>"
-  apply (case_tac cap)
-               apply ((wpsimp wp: gts_wp get_simple_ko_wp | intro conjI impI)+)
-  done
-
-lemma deleting_irq_handler_ct_not_queued[wp]:
-  "\<lbrace>ct_not_queued and scheduler_act_sane and valid_ntfn_q and valid_ep_q\<rbrace>
-   deleting_irq_handler y
-   \<lbrace>\<lambda>_. ct_not_queued :: det_state \<Rightarrow> _\<rbrace>"
-  unfolding deleting_irq_handler_def
-  by (wpsimp simp: cap_delete_one_def wp: hoare_drop_imp hoare_vcg_if_lift2)
 
 lemma unbind_from_sc_ct_not_queued[wp]:
   "\<lbrace>ct_not_queued and scheduler_act_sane\<rbrace>
@@ -6232,40 +6000,12 @@ lemma unbind_from_sc_ct_not_queued[wp]:
   unfolding unbind_from_sc_def
   by (wpsimp wp: hoare_vcg_all_lift hoare_drop_imps)
 
-lemma finalise_cap_ct_not_queued[wp]:
-  "\<lbrace>ct_not_queued and scheduler_act_sane and valid_ntfn_q and valid_ep_q\<rbrace>
-   finalise_cap cap param_b
-   \<lbrace>\<lambda>_. ct_not_queued:: det_state \<Rightarrow> _\<rbrace>"
-  apply (case_tac cap)
-               apply ((wpsimp wp: gts_wp get_simple_ko_wp | intro conjI impI)+)
-  done
-
-lemma set_sc_obj_ref_cur_sc_chargeable_const:
-  "(\<And>sc.  sc_tcb (f (\<lambda>y. val) sc) = sc_tcb sc ) \<Longrightarrow>
-   set_sc_obj_ref f scp val \<lbrace>cur_sc_chargeable\<rbrace>"
-  apply (wpsimp simp: set_sc_obj_ref_def wp: update_sched_context_wp)
-  apply (clarsimp simp: cur_sc_chargeable_def obj_at_def pred_tcb_at_def
-                        bound_sc_tcb_at_kh_def obj_at_kh_def st_tcb_at_kh_def, fastforce)
-  done
-
 lemma set_tcb_obj_ref_cur_sc_chargeable_const:
-  "(\<And>t. tcb_sched_context (f (\<lambda>y. val) t) =  tcb_sched_context t \<and>
-         tcb_state (f (\<lambda>y. val) t) =  tcb_state t) \<Longrightarrow>
+  "(\<And>t. tcb_sched_context (f (\<lambda>y. val) t) = tcb_sched_context t \<and>
+         tcb_state (f (\<lambda>y. val) t) = tcb_state t) \<Longrightarrow>
    set_tcb_obj_ref f tptr val \<lbrace>cur_sc_chargeable\<rbrace>"
   apply (wpsimp simp: set_tcb_obj_ref_def wp: set_object_wp)
-  apply (fastforce simp: cur_sc_chargeable_def obj_at_def pred_tcb_at_def
-                         bound_sc_tcb_at_kh_def obj_at_kh_def st_tcb_at_kh_def
-                  dest!: get_tcb_SomeD)
-  done
-
-lemma update_sched_context_cur_sc_chargeable_const:
-  "(\<And>x. sc_tcb (f x) = sc_tcb x) \<Longrightarrow>
-   update_sched_context ptr f \<lbrace>cur_sc_chargeable\<rbrace>"
-  apply (wpsimp simp: update_sched_context_def wp: set_object_wp get_object_wp)
-  apply (clarsimp simp: cur_sc_chargeable_def obj_at_def pred_tcb_at_def
-                         bound_sc_tcb_at_kh_def obj_at_kh_def st_tcb_at_kh_def, fastforce
-                  dest!: get_tcb_SomeD)
-  done
+  by (clarsimp simp: cur_sc_chargeable_def vs_all_heap_simps obj_at_kh_kheap_simps)
 
 lemma thread_set_cur_sc_chargeable_const:
   "(\<And>x. tcb_sched_context (f x) = tcb_sched_context x \<and>
@@ -6278,68 +6018,14 @@ lemma thread_set_cur_sc_chargeable_const:
   apply (case_tac "cur_thread s = x2"; simp, fastforce)
   done
 
-lemmas misc_cur_sc_chargeable_const = set_sc_obj_ref_cur_sc_chargeable_const
-                set_tcb_obj_ref_cur_sc_chargeable_const
-                thread_set_cur_sc_chargeable_const
-                update_sched_context_cur_sc_chargeable_const
-
-lemma update_sk_obj_ref_cur_sc_chargeable:
-  "inj C \<Longrightarrow> (\<And>x y. C x \<noteq> TCB y) \<Longrightarrow> (\<And>x y n. C x \<noteq> SchedContext y n) \<Longrightarrow>
-   update_sk_obj_ref C f ref new
-   \<lbrace>cur_sc_chargeable\<rbrace>"
-  unfolding update_sk_obj_ref_def
-  apply (wpsimp wp: set_simple_ko_wp get_simple_ko_wp)
-  apply (clarsimp simp: cur_sc_chargeable_def2 cur_sc_chargeable_def
-                        obj_at_def pred_tcb_at_def is_sc_obj_def
-                        bound_sc_tcb_at_kh_def obj_at_kh_def simple_obj_at_def st_tcb_at_kh_def, fastforce)
-  done
-
-lemma set_simple_ko_cur_sc_chargeable:
-  "inj C \<Longrightarrow> (\<And>x y. C x \<noteq> TCB y) \<Longrightarrow> (\<And>x y n. C x \<noteq> SchedContext y n) \<Longrightarrow>
-   set_simple_ko C ref new
-   \<lbrace>cur_sc_chargeable\<rbrace>"
-  unfolding update_sk_obj_ref_def
-  apply (wpsimp wp: set_simple_ko_wp get_simple_ko_wp)
-  apply (clarsimp simp: cur_sc_chargeable_def2 cur_sc_chargeable_def
-                        obj_at_def pred_tcb_at_def is_sc_obj_def
-                        bound_sc_tcb_at_kh_def obj_at_kh_def simple_obj_at_def st_tcb_at_kh_def, fastforce)
-  done
-
-crunches unbind_maybe_notification, sched_context_maybe_unbind_ntfn, unbind_notification,
-         sched_context_unbind_reply, sched_context_unbind_ntfn
-  for cur_sc_chargeable[wp]: cur_sc_chargeable
-  (ignore: set_tcb_obj_ref set_sc_obj_ref
-       wp: misc_cur_sc_chargeable_const crunch_wps)
-
-lemma sched_context_update_consumed_cur_sc_chargeable[wp]:
-  "sched_context_update_consumed x \<lbrace>cur_sc_chargeable\<rbrace>"
-  unfolding sched_context_update_consumed_def cur_sc_chargeable_def2
-  apply (wpsimp simp: update_sched_context_def wp: set_object_wp get_object_wp)
-  apply (clarsimp simp: pred_tcb_at_def sc_at_pred_def obj_at_def
-                 dest!: get_tcb_SomeD, fastforce)
-  done
-
-crunches unbind_maybe_notification, sched_context_maybe_unbind_ntfn, unbind_notification,
-         sched_context_unbind_reply, sched_context_unbind_ntfn, set_message_info, set_consumed
-  for cur_sc_chargeable[wp]: cur_sc_chargeable
-  (ignore: set_tcb_obj_ref set_sc_obj_ref
-       wp: misc_cur_sc_chargeable_const crunch_wps)
-
-lemma complete_yield_to_cur_sc_chargeable[wp]:
-  "complete_yield_to x \<lbrace>cur_sc_chargeable\<rbrace>"
-  unfolding complete_yield_to_def
-  by (wpsimp wp: misc_cur_sc_chargeable_const hoare_drop_imp)
-
-crunches tcb_release_remove, tcb_sched_action, reschedule_required
-  for cur_sc_chargeable[wp]: cur_sc_chargeable
-  (wp: crunch_wps)
+lemmas misc_cur_sc_chargeable_const =  set_tcb_obj_ref_cur_sc_chargeable_const
+                                       thread_set_cur_sc_chargeable_const
 
 lemma sched_context_unbind_tcb_cur_sc_chargeable[wp]:
   "sched_context_unbind_tcb xb \<lbrace>cur_sc_chargeable\<rbrace>"
   unfolding sched_context_unbind_tcb_def
   apply (wp)
   apply (simp add: cur_sc_chargeable_def2)
-  apply (wpsimp wp: set_sc_obj_ref_wp)
   apply (wpsimp wp: set_tcb_obj_ref_wp)
   apply (rule_tac Q="\<lambda>_. cur_sc_chargeable" in hoare_strengthen_post[rotated])
   apply (clarsimp simp: cur_sc_chargeable_def2 obj_at_def pred_tcb_at_def sc_at_pred_def, fastforce)
@@ -6350,23 +6036,6 @@ crunches sched_context_unbind_yield_from, sched_context_unbind_all_tcbs, unbind_
   for cur_sc_chargeable[wp]: cur_sc_chargeable
   (ignore: set_tcb_obj_ref set_sc_obj_ref
        wp: misc_cur_sc_chargeable_const crunch_wps maybeM_inv)
-
-crunches reply_unlink_sc
-  for cur_sc[wp]: "\<lambda>s. P (cur_sc s)"
-  (wp: crunch_wps)
-
-lemma fkh_budget_conditions_kheap_update_consthh[wp]:
-  "update_sk_obj_ref h update ref new \<lbrace>cur_sc_chargeable\<rbrace>"
-  unfolding cur_sc_chargeable_def
-  by (wpsimp wp: hoare_vcg_all_lift | wps)+
-
-lemma reply_unlink_sc_cur_sc_chargeable[wp]:
-  "\<lbrace>cur_sc_chargeable \<rbrace>
-   reply_unlink_sc sc r
-   \<lbrace>\<lambda>_. cur_sc_chargeable\<rbrace>"
-  unfolding reply_unlink_sc_def cur_sc_chargeable_def2
-  apply (wpsimp wp: hoare_vcg_all_lift hoare_vcg_imp_lift' get_simple_ko_wp | wps)+
-  by auto
 
 lemma reply_remove_cur_sc_chargeable:
   "\<lbrace>cur_sc_chargeable and cur_tcb and (\<lambda>s. t \<noteq> cur_thread s)\<rbrace>
@@ -6387,53 +6056,34 @@ lemma reply_remove_cur_sc_chargeable:
            apply (wpsimp wp: set_sc_obj_ref_wp)
           apply (rule_tac Q="\<lambda>_. cur_sc_chargeable and cur_tcb and (\<lambda>s. t \<noteq> cur_thread s)"
                  in hoare_strengthen_post[rotated])
-           apply (clarsimp simp: pred_tcb_at_def obj_at_def cur_sc_chargeable_def is_tcb
-                                 bound_sc_tcb_at_kh_def st_tcb_at_kh_def obj_at_kh_def cur_tcb_def
-                          split: if_splits, fastforce)
+           apply (clarsimp simp: obj_at_kh_kheap_simps vs_all_heap_simps cur_sc_chargeable_def pred_map_simps split: if_split, fastforce)
           apply (wpsimp simp: test_reschedule_def)
              apply (wpsimp wp: set_tcb_obj_ref_wp)
             apply (rule_tac Q="\<lambda>_. cur_sc_chargeable and cur_tcb and (\<lambda>s. t \<noteq> cur_thread s)"
                    in hoare_strengthen_post[rotated])
-             apply (clarsimp simp: pred_tcb_at_def obj_at_def cur_sc_chargeable_def is_tcb
-                                   bound_sc_tcb_at_kh_def st_tcb_at_kh_def obj_at_kh_def cur_tcb_def
-                            split: if_splits, fastforce)
+             apply (clarsimp simp: obj_at_kh_kheap_simps vs_all_heap_simps cur_sc_chargeable_def pred_map_simps cur_tcb_def is_tcb split: if_split, fastforce)
             apply (wpsimp wp: hoare_vcg_if_lift2 hoare_drop_imp)
            apply (wpsimp wp: hoare_vcg_if_lift2 hoare_drop_imp assert_opt_inv)
           apply (wpsimp wp: assert_opt_inv)
          apply (wpsimp wp: hoare_vcg_if_lift2 hoare_drop_imp)
         apply (rule_tac Q="\<lambda>_. cur_sc_chargeable and cur_tcb and (\<lambda>s. t \<noteq> cur_thread s)"
                in hoare_strengthen_post[rotated])
-         apply (clarsimp simp: pred_tcb_at_def obj_at_def cur_sc_chargeable_def is_tcb
-                               bound_sc_tcb_at_kh_def st_tcb_at_kh_def obj_at_kh_def cur_tcb_def
-                        split: if_splits)
+         apply (clarsimp simp: obj_at_kh_kheap_simps vs_all_heap_simps cur_sc_chargeable_def pred_map_simps split: if_split)
         apply (wpsimp wp: hoare_vcg_if_lift2 hoare_drop_imp)+
-  apply (clarsimp simp: pred_tcb_at_def obj_at_def cur_sc_chargeable_def is_tcb
-                        bound_sc_tcb_at_kh_def st_tcb_at_kh_def obj_at_kh_def cur_tcb_def
-                 split: if_splits)
+  apply (clarsimp simp: obj_at_kh_kheap_simps vs_all_heap_simps cur_sc_chargeable_def pred_map_simps split: if_split)
   done
 
-lemma set_thread_state_Inactive_csctb[wp]:
-  "set_thread_state d Inactive \<lbrace>cur_sc_chargeable\<rbrace>"
-  unfolding set_thread_state_def set_thread_state_act_def
-  apply (wpsimp wp: set_object_wp)
-  apply (clarsimp simp: pred_tcb_at_def obj_at_def cur_sc_chargeable_def
-                        bound_sc_tcb_at_kh_def st_tcb_at_kh_def obj_at_kh_def cur_tcb_def
-                 dest!: get_tcb_SomeD
-                 split: if_splits)
-  by fastforce
-
 lemma set_thread_state_csctb:
-  "\<lbrace>cur_sc_chargeable and (\<lambda>s. (\<forall>x. bound_sc_tcb_at (\<lambda>x. x = Some (cur_sc s)) x s \<longrightarrow> (x \<noteq> xa)))\<rbrace>
+  "\<lbrace>cur_sc_chargeable and (\<lambda>s. (\<forall>x. bound_sc_tcb_at (\<lambda>x. x = Some (cur_sc s)) x s \<longrightarrow> (x \<noteq> xa \<or> d = Inactive)))\<rbrace>
    set_thread_state xa d
    \<lbrace>\<lambda>xa. cur_sc_chargeable\<rbrace>"
   unfolding set_thread_state_def set_thread_state_act_def
   apply (wpsimp wp: set_object_wp)
-  apply (clarsimp simp: pred_tcb_at_def obj_at_def cur_sc_chargeable_def
-                        bound_sc_tcb_at_kh_def st_tcb_at_kh_def obj_at_kh_def cur_tcb_def
-                 dest!: get_tcb_SomeD
-                 split: if_splits)
-  by fastforce
+  by (clarsimp simp: obj_at_kh_kheap_simps vs_all_heap_simps cur_sc_chargeable_def)
 
+lemma set_thread_state_Inactive_csctb[wp]:
+  "set_thread_state d Inactive \<lbrace>cur_sc_chargeable\<rbrace>"
+  by (wpsimp wp: set_thread_state_csctb)
 
 lemma restart_thread_if_no_fault_csctb:
   "\<lbrace>cur_sc_chargeable and (\<lambda>s. (\<forall>x. bound_sc_tcb_at (\<lambda>x. x = Some (cur_sc s)) x s \<longrightarrow> (x \<noteq> xa)))\<rbrace>
@@ -6448,52 +6098,32 @@ lemma reply_unlink_tcb_csctb:
    \<lbrace>\<lambda>_. cur_sc_chargeable\<rbrace>"
   unfolding reply_unlink_tcb_def
   apply (wpsimp wp: set_thread_state_csctb update_sk_obj_ref_wp gts_wp get_simple_ko_wp)
-  apply (clarsimp simp: pred_tcb_at_def obj_at_def cur_sc_chargeable_def
-                        bound_sc_tcb_at_kh_def st_tcb_at_kh_def obj_at_kh_def cur_tcb_def
-                 dest!: get_tcb_SomeD
-                 split: if_splits)
-  by fastforce
-
-lemma valid_ntfn_q_Blocked:
-  "valid_ntfn_q (s:: det_state) \<Longrightarrow>
-   (\<forall>p. case kheap s p of Some (Notification n) \<Rightarrow>
-      \<forall>t \<in> set (ntfn_queue n). st_tcb_at (Not \<circ> not_blocked) t s
-           | _ \<Rightarrow> True)"
-  unfolding valid_ntfn_q_def2
-  apply (clarsimp split: option.splits)
-  apply (case_tac x2; clarsimp)
-  apply (clarsimp simp: simple_obj_at_def)
-  apply (drule_tac x=t and y=p in spec2, clarsimp)
-  by (clarsimp simp: pred_tcb_at_def obj_at_def)
+  by (clarsimp simp: obj_at_kh_kheap_simps vs_all_heap_simps cur_sc_chargeable_def)
 
 lemma restart_thread_if_no_fault_not_bound_sc_tcb_at[wp]:
   "restart_thread_if_no_fault x \<lbrace>\<lambda>s. \<not> bound_sc_tcb_at P xs s\<rbrace>"
   unfolding restart_thread_if_no_fault_def
   by wpsimp
 
-(* fixme: move *)
-abbreviation
-  "Blocked st \<equiv> (Not \<circ> not_blocked) st"
-
-lemma cancel_all_ipc_cur_sc_chargeable:
-  "\<lbrace>cur_sc_chargeable and valid_ep_q\<rbrace>
+lemma cancel_all_ipc_cur_thread_on_preemption:
+  "\<lbrace>cur_thread_on_preemption and schedulable_ipc_queues and invs and scheduler_act_sane and ct_not_blocked\<rbrace>
    cancel_all_ipc x
-   \<lbrace>\<lambda>_. cur_sc_chargeable\<rbrace>"
-  unfolding cancel_all_ipc_def
+   \<lbrace>\<lambda>_. cur_thread_on_preemption\<rbrace>"
+  unfolding cancel_all_ipc_def cur_thread_on_preemption_def
   apply wpsimp
-      apply (rule_tac R="\<lambda>_ s. \<forall>x \<in> set queue. \<not> bound_sc_tcb_at (\<lambda>x. x = Some (cur_sc s)) x s" in hoare_post_add)
-      apply (rule mapM_x_wp[where S="set xs" and xs=xs for xs])
-       apply wpsimp
-           apply ((wpsimp wp: restart_thread_if_no_fault_csctb hoare_vcg_ball_lift restart_thread_if_no_fault_other reply_unlink_tcb_csctb
-                              hoare_vcg_all_lift hoare_vcg_imp_lift'
-                   | rule hoare_lift_Pf[where f = cur_sc])+)[3]
-        apply (wp gts_wp)
-       apply (clarsimp)
-       apply (drule_tac x=x in bspec, simp)
-       apply (intro conjI; clarsimp)
+       apply (rule_tac R="\<lambda>_ s. \<forall>x \<in> set queue. \<not> bound_sc_tcb_at (\<lambda>x. x = Some (cur_sc s)) x s \<and> x \<noteq> cur_thread s" in hoare_post_add)
+       apply (rule mapM_x_wp[where S="set xs" and xs=xs for xs])
+        apply wpsimp
+            apply ((wpsimp wp: restart_thread_if_no_fault_csctb hoare_vcg_ball_lift restart_thread_if_no_fault_other reply_unlink_tcb_csctb
+                               hoare_vcg_all_lift hoare_vcg_imp_lift'
+                    | rule hoare_lift_Pf[where f = cur_sc])+)[3]
+         apply (wp gts_wp)
+        apply (clarsimp)
+        apply (drule_tac x=x in bspec, simp)
+        apply (intro conjI; clarsimp)
        apply clarsimp
       apply (wpsimp wp: set_simple_ko_wp get_ep_queue_wp)+
-      apply (rule_tac R="\<lambda>_ s. \<forall>x \<in> set queue. \<not> bound_sc_tcb_at (\<lambda>x. x = Some (cur_sc s)) (x) s" in hoare_post_add)
+      apply (rule_tac R="\<lambda>_ s. \<forall>x \<in> set queue. \<not> bound_sc_tcb_at (\<lambda>x. x = Some (cur_sc s)) x s \<and> x \<noteq> cur_thread s" in hoare_post_add)
       apply (rule mapM_x_wp[where S="set xs" and xs=xs for xs])
        apply wpsimp
            apply ((wpsimp wp: restart_thread_if_no_fault_csctb hoare_vcg_ball_lift restart_thread_if_no_fault_other reply_unlink_tcb_csctb
@@ -6503,76 +6133,58 @@ lemma cancel_all_ipc_cur_sc_chargeable:
        apply (clarsimp)
        apply (drule_tac x=x in bspec, simp)
        apply (intro conjI; clarsimp)
-       apply clarsimp
-      apply (wpsimp wp: set_simple_ko_wp get_ep_queue_wp get_simple_ko_wp)+
+      apply clarsimp
+     apply (wpsimp wp: set_simple_ko_wp get_ep_queue_wp get_simple_ko_wp)+
   apply (intro conjI; intro allI impI; intro conjI)
-    apply (clarsimp)
-    apply (subgoal_tac "st_tcb_at Blocked xaa s \<and> (xaa \<noteq> cur_thread s)")
-        apply (clarsimp simp: obj_at_def cur_sc_chargeable_2_def pred_tcb_at_def
-                              bound_sc_tcb_at_kh_def obj_at_kh_def ep_at_pred_def pred_neg_def
-                       split: if_splits
-               , fastforce)
-      apply (clarsimp simp: valid_ep_q_def2 pred_neg_def pred_tcb_at_def obj_at_def simple_obj_at_def, fastforce)
-    apply (clarsimp simp: obj_at_def cur_sc_chargeable_2_def pred_tcb_at_def st_tcb_at_kh_def
-                          bound_sc_tcb_at_kh_def obj_at_kh_def ep_at_pred_def pred_neg_def
-                   split: if_splits
-           , fastforce)
-    apply (clarsimp)
-    apply (subgoal_tac "st_tcb_at Blocked xaa s \<and> (xaa \<noteq> cur_thread s)")
-        apply (clarsimp simp: obj_at_def cur_sc_chargeable_2_def pred_tcb_at_def
-                              bound_sc_tcb_at_kh_def obj_at_kh_def ep_at_pred_def pred_neg_def
-                       split: if_splits
-               , fastforce)
-      apply (clarsimp simp: valid_ep_q_def2 pred_neg_def pred_tcb_at_def obj_at_def simple_obj_at_def, fastforce)
-    apply (clarsimp simp: obj_at_def cur_sc_chargeable_2_def pred_tcb_at_def st_tcb_at_kh_def
-                          bound_sc_tcb_at_kh_def obj_at_kh_def ep_at_pred_def pred_neg_def
-                   split: if_splits
-           , fastforce)
-done
+     apply (clarsimp simp: obj_at_def)
+     apply (subgoal_tac "ipc_queued_thread xaa s")
+      apply (subgoal_tac "(xaa \<noteq> cur_thread s)")
+       apply (clarsimp simp: obj_at_kh_kheap_simps cur_sc_chargeable_def pred_map_simps, fastforce)
+      apply (clarsimp simp: obj_at_kh_kheap_simps ct_in_state_kh_simp pred_map_simps)
+     apply (erule sym_refs_SendEP_ipc_queued_thread; clarsimp)
+    apply (clarsimp simp:  cur_sc_chargeable_def vs_all_heap_simps)
+   apply (clarsimp simp: obj_at_def)
+   apply (subgoal_tac "ipc_queued_thread xaa s")
+    apply (subgoal_tac "(xaa \<noteq> cur_thread s)")
+     apply (clarsimp simp: obj_at_kh_kheap_simps cur_sc_chargeable_def pred_map_simps, fastforce)
+    apply (clarsimp simp: obj_at_kh_kheap_simps ct_in_state_kh_simp pred_map_simps)
+   apply (erule sym_refs_RecvEP_ipc_queued_thread; clarsimp)
+  apply (clarsimp simp:  cur_sc_chargeable_def vs_all_heap_simps)
+  done
 
-lemma possible_switch_to_cur_sc_chargeable[wp]:
-  "possible_switch_to x \<lbrace>cur_sc_chargeable\<rbrace>"
-  unfolding possible_switch_to_def
-  by (wpsimp wp: hoare_drop_imp)
-
-lemma cancel_all_signals_cur_sc_chargeable:
-  "\<lbrace>cur_sc_chargeable and valid_ntfn_q\<rbrace>
+lemma cancel_all_signals_cur_thread_on_preemption:
+  "\<lbrace>cur_thread_on_preemption and schedulable_ipc_queues and invs and ct_not_blocked and scheduler_act_sane\<rbrace>
    cancel_all_signals x
-   \<lbrace>\<lambda>_. cur_sc_chargeable :: det_state \<Rightarrow> _\<rbrace>"
-  unfolding cancel_all_signals_def
+   \<lbrace>\<lambda>_. cur_thread_on_preemption :: det_state \<Rightarrow> _\<rbrace>"
+  unfolding cancel_all_signals_def cur_thread_on_preemption_def
   apply wpsimp
-      apply (rule_tac R="\<lambda>_ s. \<forall>x \<in> set x2. \<not> bound_sc_tcb_at (\<lambda>x. x = Some (cur_sc s)) (x) s" in hoare_post_add)
+      apply (rule_tac R="\<lambda>_ s. \<forall>x \<in> set x2. \<not> bound_sc_tcb_at (\<lambda>x. x = Some (cur_sc s)) (x) s \<and> x \<noteq> cur_thread s" in hoare_post_add)
       apply (rule mapM_x_wp[where S="set xs" and xs=xs for xs])
-      apply (wpsimp wp: hoare_vcg_ball_lift hoare_vcg_all_lift hoare_vcg_imp_lift' set_thread_state_csctb sts_st_tcb_at_other)
-      apply (wps, wpsimp)
-      apply (wps, wpsimp)
-      apply (wpsimp wp: hoare_vcg_ball_lift hoare_vcg_all_lift hoare_vcg_imp_lift' set_thread_state_csctb sts_st_tcb_at_other)
-      apply (intro conjI; clarsimp)
+       apply (wpsimp wp: hoare_vcg_ball_lift hoare_vcg_all_lift hoare_vcg_imp_lift' set_thread_state_csctb sts_st_tcb_at_other)
+          apply (wps, wpsimp)
+         apply (wps, wpsimp)
+        apply (wpsimp wp: hoare_vcg_ball_lift hoare_vcg_all_lift hoare_vcg_imp_lift' set_thread_state_csctb sts_st_tcb_at_other
+                          possible_switch_to_ct_not_queued possible_switch_to_scheduler_act_sane')
+       apply (intro conjI; clarsimp)
       apply simp
      apply (wpsimp wp: set_simple_ko_wp get_simple_ko_wp)+
   apply (intro conjI)
-    apply clarsimp
-    apply (subgoal_tac "st_tcb_at Blocked xaa s \<and> (xaa \<noteq> cur_thread s)")
-
-    apply (clarsimp simp: obj_at_def cur_sc_chargeable_2_def pred_tcb_at_def
-   bound_sc_tcb_at_kh_def obj_at_kh_def ep_at_pred_def pred_neg_def split: if_splits, fastforce)
-      apply (clarsimp simp: valid_ntfn_q_def2 pred_neg_def pred_tcb_at_def obj_at_def simple_obj_at_def ntfn_queue_def
-                     split: if_splits
-             , fastforce)
-    apply (clarsimp simp: obj_at_def cur_sc_chargeable_2_def pred_tcb_at_def
-                          bound_sc_tcb_at_kh_def obj_at_kh_def ep_at_pred_def pred_neg_def st_tcb_at_kh_def
-                   split: if_splits
-           , fastforce)
+   apply (clarsimp simp: obj_at_def)
+   apply (subgoal_tac "ipc_queued_thread xaa s")
+    apply (subgoal_tac "(xaa \<noteq> cur_thread s)")
+     apply (clarsimp simp: obj_at_kh_kheap_simps cur_sc_chargeable_def pred_map_simps, fastforce)
+    apply (clarsimp simp: obj_at_kh_kheap_simps ct_in_state_kh_simp pred_map_simps)
+   apply (erule sym_refs_WaitingNtfn_ipc_queued_thread, assumption, clarsimp, clarsimp)
+  apply (clarsimp simp:  cur_sc_chargeable_def vs_all_heap_simps)
   done
 
 lemma blocked_cancel_ipc_cur_sc_chargeable:
-  "\<lbrace>cur_sc_chargeable and (\<lambda>s. x\<noteq>cur_thread s) and st_tcb_at (not inactive) x\<rbrace>
+  "\<lbrace>cur_sc_chargeable and (\<lambda>s. x\<noteq>cur_thread s) and st_tcb_at (Not \<circ> inactive) x\<rbrace>
    blocked_cancel_ipc a x c
    \<lbrace>\<lambda>_. cur_sc_chargeable\<rbrace>"
   unfolding blocked_cancel_ipc_def
   apply (wpsimp wp: reply_unlink_tcb_csctb get_simple_ko_wp set_simple_ko_wp get_ep_queue_wp get_blocking_object_wp)
-  apply (clarsimp simp: cur_sc_chargeable_def pred_tcb_at_def obj_at_def bound_sc_tcb_at_kh_def obj_at_kh_def
-                        cur_tcb_def is_tcb pred_neg_def)
+  apply (clarsimp simp: obj_at_kh_kheap_simps vs_all_heap_simps cur_sc_chargeable_def)
   by fastforce
 
 lemma reply_remove_tcb_cur_sc_chargeable:
@@ -6581,8 +6193,7 @@ lemma reply_remove_tcb_cur_sc_chargeable:
    \<lbrace>\<lambda>_. cur_sc_chargeable\<rbrace>"
   unfolding reply_remove_tcb_def
   apply (wpsimp wp: reply_unlink_tcb_csctb update_sk_obj_ref_wp update_sched_context_wp get_sk_obj_ref_wp gts_wp)
-  apply (clarsimp simp: cur_sc_chargeable_def pred_tcb_at_def obj_at_def bound_sc_tcb_at_kh_def obj_at_kh_def
-                    cur_tcb_def is_tcb pred_neg_def st_tcb_at_kh_def)
+  apply (clarsimp simp: obj_at_kh_kheap_simps vs_all_heap_simps cur_sc_chargeable_def)
   by fastforce
 
 lemma cancel_signal_cur_sc_chargeable:
@@ -6591,17 +6202,14 @@ lemma cancel_signal_cur_sc_chargeable:
    \<lbrace>\<lambda>_. cur_sc_chargeable\<rbrace>"
   unfolding cancel_signal_def
   apply (wpsimp wp: reply_unlink_tcb_csctb set_simple_ko_wp get_simple_ko_wp)
-  by (fastforce simp: cur_sc_chargeable_def pred_tcb_at_def obj_at_def bound_sc_tcb_at_kh_def obj_at_kh_def
-                      cur_tcb_def is_tcb pred_neg_def st_tcb_at_kh_def)
+  by (clarsimp simp: obj_at_kh_kheap_simps vs_all_heap_simps cur_sc_chargeable_def)
 
 lemma thread_set_cur_sc_chargeable_indep:
   "\<forall>tcb. tcb_sched_context (a tcb) = tcb_sched_context (tcb) \<Longrightarrow>
    \<forall>tcb. tcb_state (a tcb) = tcb_state tcb \<Longrightarrow>
    thread_set a b \<lbrace>cur_sc_chargeable\<rbrace>"
   apply (wpsimp wp: thread_set_wp)
-  apply (clarsimp simp: cur_sc_chargeable_def pred_tcb_at_def obj_at_def bound_sc_tcb_at_kh_def obj_at_kh_def
-                    cur_tcb_def is_tcb pred_neg_def st_tcb_at_kh_def ct_in_state_def
-              dest!: get_tcb_SomeD)
+  apply (clarsimp simp: obj_at_kh_kheap_simps vs_all_heap_simps cur_sc_chargeable_def)
   by fastforce
 
 lemma cancel_ipc_cur_sc_chargeable2:
@@ -6611,14 +6219,11 @@ lemma cancel_ipc_cur_sc_chargeable2:
   unfolding cancel_ipc_def
   apply (wpsimp wp: blocked_cancel_ipc_cur_sc_chargeable reply_remove_tcb_cur_sc_chargeable
                     cancel_signal_cur_sc_chargeable)
-  apply (wpsimp wp: thread_set_cur_sc_chargeable_indep hoare_vcg_imp_lift' gts_wp thread_set_no_change_tcb_state)+
+    apply (wpsimp wp: thread_set_cur_sc_chargeable_indep hoare_vcg_imp_lift' gts_wp thread_set_no_change_tcb_state)+
   apply (case_tac "x = cur_thread s")
-  apply (clarsimp simp: cur_sc_chargeable_def pred_tcb_at_def obj_at_def bound_sc_tcb_at_kh_def obj_at_kh_def
-                    cur_tcb_def is_tcb pred_neg_def st_tcb_at_kh_def ct_in_state_def
-              dest!: get_tcb_SomeD)
-  apply (fastforce)
-  apply (clarsimp simp: pred_neg_def pred_tcb_at_def obj_at_def)
-  apply (fastforce)
+   apply (clarsimp simp: obj_at_kh_kheap_simps vs_all_heap_simps cur_sc_chargeable_def ct_in_state_def
+          , fastforce)
+  apply (fastforce simp: tcb_at_kh_simps vs_all_heap_simps)
   done
 
 lemma cancel_ipc_cur_sc_chargeable:
@@ -6629,75 +6234,54 @@ lemma cancel_ipc_cur_sc_chargeable:
   apply (wpsimp wp: blocked_cancel_ipc_cur_sc_chargeable
                     reply_remove_tcb_cur_sc_chargeable
                     cancel_signal_cur_sc_chargeable thread_set_wp gts_wp)
-  by (fastforce simp: cur_sc_chargeable_def pred_tcb_at_def obj_at_def bound_sc_tcb_at_kh_def obj_at_kh_def
-                      cur_tcb_def is_tcb pred_neg_def st_tcb_at_kh_def
-               dest!: get_tcb_SomeD)
+  by (fastforce simp: cur_sc_chargeable_def obj_at_kh_kheap_simps vs_all_heap_simps)
 
-lemma fast_finalise_cur_sc_chargeable:
-  "\<lbrace>cur_sc_chargeable and valid_ep_q and valid_ntfn_q and invs
-     and ct_not_blocked \<rbrace>
+crunches cancel_ipc, reply_remove, sched_context_unbind_all_tcbs, suspend, unbind_from_sc
+  for ct_not_in_release_q[wp]: "ct_not_in_release_q :: det_state \<Rightarrow> _"
+  (wp: crunch_wps hoare_vcg_all_lift)
+
+lemma fast_finalise_cur_thread_on_preemption:
+  "\<lbrace>cur_thread_on_preemption and schedulable_ipc_queues and invs and scheduler_act_sane and ct_not_blocked \<rbrace>
    fast_finalise d e
-   \<lbrace>\<lambda>_. cur_sc_chargeable :: det_state \<Rightarrow> _\<rbrace>"
+   \<lbrace>\<lambda>_. cur_thread_on_preemption :: det_state \<Rightarrow> _\<rbrace>"
   apply (case_tac d; simp)
       apply wpsimp
-     apply (wpsimp wp: cancel_all_ipc_cur_sc_chargeable)
-    apply (wpsimp wp: cancel_all_signals_cur_sc_chargeable)
-   subgoal for x5
-   apply (wpsimp wp: cancel_ipc_cur_sc_chargeable2 reply_remove_cur_sc_chargeable)
+     apply (wpsimp wp: cancel_all_ipc_cur_thread_on_preemption)
+    apply (wpsimp wp: cancel_all_signals_cur_thread_on_preemption unbind_maybe_notification_invs simp: cur_thread_on_preemption_def)
+   subgoal for rcap
+   apply (simp add: cur_thread_on_preemption_def)
+   apply (wpsimp wp: cancel_ipc_cur_sc_chargeable reply_remove_cur_sc_chargeable)
      apply (wpsimp wp: gts_wp get_simple_ko_wp)+
-   apply (subgoal_tac "st_tcb_at (not not_blocked) x s")
-    apply (fastforce simp: ct_in_state_def pred_tcb_at_def pred_neg_def obj_at_def)
-   apply (subgoal_tac "(x5, TCBReply) \<in> state_refs_of s x")
+   apply (subgoal_tac "st_tcb_at (ipc_queued_thread_state) x s")
+    apply (clarsimp simp: obj_at_kh_kheap_simps ct_in_state_kh_simp)
+   apply (intro conjI; intro allI impI; clarsimp simp: invs_def pred_map_simps)
+   apply (subgoal_tac "(rcap, TCBReply) \<in> state_refs_of s x")
     apply (clarsimp simp: pred_tcb_at_def obj_at_def state_refs_of_def get_refs_def2 tcb_st_refs_of_def
                           pred_neg_def
                    split: thread_state.splits if_splits)
    apply (erule reply_tcb_not_idle_thread_helper, simp add: obj_at_def, clarsimp)
    done
-  apply (wpsimp wp: set_sc_obj_ref_cur_sc_chargeable_const)
+  apply (wpsimp simp: cur_thread_on_preemption_def)
   done
 
-lemma set_cap_cur_sc_chargeablep[wp]:
-  "\<lbrace>cur_sc_chargeable\<rbrace>
-   set_cap d a
-   \<lbrace>\<lambda>_. cur_sc_chargeable :: det_state \<Rightarrow> _\<rbrace>"
-   unfolding set_cap_def
-   apply (wpsimp wp: set_object_wp get_object_wp)
-   by (fastforce simp: cur_sc_chargeable_def bound_sc_tcb_at_kh_def obj_at_kh_def
-                         obj_at_def st_tcb_at_kh_def)
+lemma empty_slot_cur_thread_on_preemption[wp]:
+  "empty_slot slot cleanup_info \<lbrace>cur_thread_on_preemption :: det_state \<Rightarrow> _\<rbrace>"
+  by (wpsimp simp: cur_thread_on_preemption_def)
 
-lemma set_cdt_cur_sc_chargeablep[wp]:
-  "\<lbrace>cur_sc_chargeable\<rbrace>
-   set_cdt d
-   \<lbrace>\<lambda>_. cur_sc_chargeable :: det_state \<Rightarrow> _\<rbrace>"
-   unfolding set_cdt_def
-   by (wpsimp wp: set_object_wp get_object_wp)
-
-crunches empty_slot
-  for cur_sc_chargeable[wp]: "cur_sc_chargeable :: det_state \<Rightarrow> _"
-  (ignore: set_tcb_obj_ref set_sc_obj_ref
-       wp: misc_cur_sc_chargeable_const crunch_wps simp: crunch_simps)
-
-lemma cap_delete_one_cur_sc_chargeable:
-  "\<lbrace>cur_sc_chargeable and invs and ct_not_blocked and valid_ep_q and valid_ntfn_q\<rbrace>
+lemma cap_delete_one_cur_thread_on_preemption[wp]:
+  "\<lbrace>cur_thread_on_preemption and invs and ct_not_blocked and schedulable_ipc_queues and scheduler_act_sane\<rbrace>
    cap_delete_one d
-   \<lbrace>\<lambda>_. cur_sc_chargeable :: det_state \<Rightarrow> _\<rbrace>"
+   \<lbrace>\<lambda>_. cur_thread_on_preemption :: det_state \<Rightarrow> _\<rbrace>"
   unfolding cap_delete_one_def
-  by (wpsimp wp: get_cap_wp fast_finalise_cur_sc_chargeable)
-
-crunches deleting_irq_handler
-  for cur_sc_chargeable[wp]: "cur_sc_chargeable :: det_state \<Rightarrow> _"
-  (ignore: set_tcb_obj_ref set_sc_obj_ref
-       wp: misc_cur_sc_chargeable_const crunch_wps simp: crunch_simps)
+  by (wpsimp wp: get_cap_wp fast_finalise_cur_thread_on_preemption)
 
 lemma suspend_cur_sc_chargeable:
   "\<lbrace>cur_sc_chargeable and ct_not_blocked\<rbrace>
    suspend x
    \<lbrace>\<lambda>_. cur_sc_chargeable :: det_state \<Rightarrow> _\<rbrace>"
   unfolding suspend_def
-  apply (wpsimp wp: set_tcb_obj_ref_cur_sc_chargeable_const
-                    set_sc_obj_ref_cur_sc_chargeable_const hoare_drop_imp
+  by (wpsimp wp: set_tcb_obj_ref_cur_sc_chargeable_const hoare_drop_imp
                     cancel_ipc_cur_sc_chargeable2)
-  done
 
 (* FIXME: set_tcb_obj_ref does more than set tcb object references *)
 
@@ -6713,64 +6297,64 @@ crunches unbind_from_sc, unbind_notification
   for ct_in_state[wp]: "ct_in_state P"
   (wp: crunch_wps hoare_drop_imp hoare_vcg_all_lift)
 
-lemma finalise_cap_cur_sc_chargeable[wp]:
-  "\<lbrace>cur_sc_chargeable and invs and ct_not_blocked and valid_ep_q and valid_ntfn_q\<rbrace>
+lemma unbind_maybe_notification_cur_thread_on_preemption[wp]:
+  "unbind_maybe_notification d \<lbrace>cur_thread_on_preemption\<rbrace>"
+  by (wpsimp simp: cur_thread_on_preemption_def )
+
+lemma cancel_ipc_cur_thread_on_preemption[wp]:
+  "\<lbrace>cur_thread_on_preemption and cur_tcb and (\<lambda>s. tp \<noteq> cur_thread s)\<rbrace>
+   cancel_ipc tp
+   \<lbrace>\<lambda>_. cur_thread_on_preemption :: det_state \<Rightarrow> _\<rbrace>"
+  by (wpsimp simp: cur_thread_on_preemption_def wp: cancel_ipc_cur_sc_chargeable)
+
+lemma reply_remove_cur_thread_on_preemption[wp]:
+  "\<lbrace>cur_thread_on_preemption and scheduler_act_sane and cur_tcb and (\<lambda>s. tp \<noteq> cur_thread s)\<rbrace>
+   reply_remove tp r
+   \<lbrace>\<lambda>_. cur_thread_on_preemption :: det_state \<Rightarrow> _\<rbrace>"
+  by (wpsimp simp: cur_thread_on_preemption_def wp: reply_remove_cur_sc_chargeable)
+
+lemma sched_context_maybe_unbind_ntfn_cur_thread_on_preemption[wp]:
+  "sched_context_maybe_unbind_ntfn d \<lbrace>cur_thread_on_preemption\<rbrace>"
+  by (wpsimp simp: cur_thread_on_preemption_def)
+
+lemma deleting_irq_handler_cur_thread_on_preemption[wp]:
+  "\<lbrace>cur_thread_on_preemption and invs and ct_not_blocked and schedulable_ipc_queues and scheduler_act_sane\<rbrace>
+   deleting_irq_handler x12
+   \<lbrace>\<lambda>_. cur_thread_on_preemption :: det_state \<Rightarrow> _\<rbrace>"
+  unfolding deleting_irq_handler_def
+  by wpsimp
+
+lemma finalise_cap_cur_thread_on_preemption:
+  "\<lbrace>cur_thread_on_preemption and invs and ct_not_blocked and schedulable_ipc_queues and scheduler_act_sane\<rbrace>
    finalise_cap d f
-   \<lbrace>\<lambda>_. cur_sc_chargeable :: det_state \<Rightarrow> _\<rbrace>"
+   \<lbrace>\<lambda>_. cur_thread_on_preemption :: det_state \<Rightarrow> _\<rbrace>"
   supply if_split [split del]
   apply (case_tac d; simp)
                apply wpsimp
               apply wpsimp
-             apply (wpsimp wp: cancel_all_ipc_cur_sc_chargeable)
-             apply (clarsimp split: if_split)
-            apply (wpsimp wp: cancel_all_signals_cur_sc_chargeable)
-            apply (clarsimp split: if_split)
-           apply (wpsimp wp: cancel_ipc_cur_sc_chargeable reply_remove_cur_sc_chargeable
-                             gts_wp get_simple_ko_wp)
-           apply (clarsimp split: if_split)
-           apply (subgoal_tac "st_tcb_at (not not_blocked) x s")
-            apply (fastforce simp: ct_in_state_def pred_tcb_at_def pred_neg_def obj_at_def)
+             apply (wpsimp wp: cancel_all_ipc_cur_thread_on_preemption split: if_split)
+            apply (wpsimp wp: cancel_all_signals_cur_thread_on_preemption unbind_maybe_notification_invs split: if_split)
+           apply (wpsimp wp: reply_remove_cur_sc_chargeable
+                             gts_wp get_simple_ko_wp split: if_split)
+   apply (subgoal_tac "st_tcb_at (ipc_queued_thread_state) x s")
+    apply (clarsimp simp: obj_at_kh_kheap_simps ct_in_state_kh_simp)
+   apply (intro conjI; intro allI impI; clarsimp simp: invs_def pred_map_simps)
            apply (subgoal_tac "(x5, TCBReply) \<in> state_refs_of s x")
             apply (clarsimp simp: pred_tcb_at_def obj_at_def state_refs_of_def get_refs_def2 tcb_st_refs_of_def
                                   pred_neg_def
                            split: thread_state.splits if_splits)
            apply (erule reply_tcb_not_idle_thread_helper, simp add: obj_at_def, clarsimp)
           apply wpsimp
-         apply (wpsimp wp: suspend_cur_sc_chargeable)
-         apply (clarsimp split: if_split)
+         apply (wpsimp simp: cur_thread_on_preemption_def wp: suspend_cur_sc_chargeable split: if_split)
         apply wpsimp
-       apply (wpsimp wp: set_sc_obj_ref_cur_sc_chargeable_const)
-      apply wpsimp+
-  done
-
-crunches complete_yield_to, sched_context_unbind_tcb
-  for ct_not_in_release_q[wp]: "ct_not_in_release_q :: det_state \<Rightarrow> _"
-  (wp: crunch_wps simp: crunch_simps)
-
-lemma unbind_from_sc_ct_not_in_release_q[wp]:
-  "\<lbrace>ct_not_in_release_q\<rbrace> unbind_from_sc param_a \<lbrace>\<lambda>_. ct_not_in_release_q:: det_state \<Rightarrow> _\<rbrace>"
-  unfolding unbind_from_sc_def
-  apply (wpsimp wp: hoare_vcg_all_lift hoare_drop_imp)
+       apply (wpsimp split: if_split simp: cur_thread_on_preemption_def)
+      apply (wpsimp)+
+  apply (wpsimp simp: cur_thread_on_preemption_def)
   done
 
 crunches finalise_cap
   for ct_not_in_release_q[wp]: "ct_not_in_release_q :: det_state \<Rightarrow> _"
   (wp: crunch_wps simp: crunch_simps)
-
-crunches cap_swap_for_delete
-  for valid_ep_q[wp]: "valid_ep_q:: det_state \<Rightarrow> _"
-  and valid_ntfn_q[wp]: "valid_ntfn_q :: det_state \<Rightarrow> _"
-
-crunches empty_slot
-  for valid_ep_q[wp]: "valid_ep_q:: det_state \<Rightarrow> _"
-  and valid_ntfn_q[wp]: "valid_ntfn_q :: det_state \<Rightarrow> _"
-
-lemma set_x_obj_ref_ep_at_pred[wp]:
-  "set_tcb_obj_ref f x v \<lbrace>\<lambda>s. Q (ep_at_pred P p s)\<rbrace>"
-  "set_sc_obj_ref a b c \<lbrace>\<lambda>s. Q (ep_at_pred P p s)\<rbrace>"
-  apply (wpsimp wp: set_tcb_obj_ref_wp, erule back_subst[where P=Q], clarsimp simp: simple_obj_at_def obj_at_def)
-  apply (wpsimp wp: set_sc_obj_ref_wp, erule back_subst[where P=Q], clarsimp simp: simple_obj_at_def obj_at_def)
-  done
 
 lemma set_tcb_pred_tcb_const:
   "(\<And>tcb. P (proj (tcb_to_itcb (f (\<lambda>y. v) tcb))) = P (proj (tcb_to_itcb tcb))) \<Longrightarrow>
@@ -6779,199 +6363,22 @@ lemma set_tcb_pred_tcb_const:
   apply (erule back_subst[where P=Q])
   by (clarsimp simp: pred_tcb_at_def obj_at_def)
 
-lemma set_tcb_active_sc_tcb_at_const:
-  "(\<And>tcb. (tcb_sched_context ( (f (\<lambda>y. v) tcb))) = (tcb_sched_context ( tcb)) ) \<Longrightarrow>
-   set_tcb_obj_ref f x v \<lbrace>active_sc_tcb_at t\<rbrace>"
-  apply (wpsimp wp: set_tcb_obj_ref_wp)
-  apply (clarsimp simp: active_sc_tcb_at_def obj_at_def pred_tcb_at_def test_sc_refill_max_def
-                 split: option.splits, fastforce)
-  done
-
-lemma set_tcb_budget_ready_const:
-  "(\<And>tcb. (tcb_sched_context ( (f (\<lambda>y. v) tcb))) = (tcb_sched_context ( tcb)) ) \<Longrightarrow>
-   set_tcb_obj_ref f x v \<lbrace>budget_ready t\<rbrace>"
-  apply (wpsimp wp: set_tcb_obj_ref_wp)
-  apply (clarsimp simp: budget_ready_defs obj_at_def pred_tcb_at_def
-                 split: option.splits)
-  apply auto
-  apply (rule_tac x=scp in exI, simp)
-  apply fastforce
-  apply (rule_tac x=scp in exI, simp)
-  apply fastforce
-  done
-
-lemma set_tcb_budget_sufficient_const:
-  "(\<And>tcb. (tcb_sched_context ( (f (\<lambda>y. v) tcb))) = (tcb_sched_context ( tcb)) ) \<Longrightarrow>
-   set_tcb_obj_ref f x v \<lbrace>budget_sufficient t\<rbrace>"
-  apply (wpsimp wp: set_tcb_obj_ref_wp)
-  apply (clarsimp simp: budget_sufficient_defs obj_at_def pred_tcb_at_def
-                 split: option.splits)
-  apply auto
-  apply (rule_tac x=scp in exI, simp)
-  apply fastforce
-  apply (rule_tac x=scp in exI, simp)
-  apply fastforce
-  done
-
 lemmas set_tcb_obj_ref_budget_ready_indep = set_tcb_pred_tcb_const
                                             set_tcb_budget_sufficient_const
                                             set_tcb_active_sc_tcb_at_const
-                                            set_tcb_budget_ready_const
-
-lemma set_tcb_obj_ref_valid_ep_q_const:
-  "(\<And>tcb.  (tcb_state ( tcb)) =  (tcb_state ( (f (\<lambda>y. v) tcb)))) \<Longrightarrow>
-   (\<And>tcb.  (tcb_sched_context ( tcb)) =  (tcb_sched_context ( (f (\<lambda>y. v) tcb)))) \<Longrightarrow>
-   set_tcb_obj_ref f x v \<lbrace>valid_ep_q\<rbrace>"
-  apply (wpsimp simp: valid_ep_q_def2)
-  apply (wpsimp wp: hoare_vcg_all_lift hoare_vcg_imp_lift' set_tcb_pred_tcb_const hoare_vcg_disj_lift
-                    set_tcb_obj_ref_budget_ready_indep)
-  done
-
-lemma set_sc_obj_ref_valid_ep_q_const:
-  "(\<And>sc. sc_refill_max (f (\<lambda>a. v) sc) = sc_refill_max sc) \<Longrightarrow>
-   (\<And>sc. sc_refills (f (\<lambda>a. v) sc) = sc_refills sc) \<Longrightarrow>
-   set_sc_obj_ref f x v \<lbrace>valid_ep_q:: det_state \<Rightarrow> _\<rbrace>"
-  apply (wpsimp simp: valid_ep_q_def2)
-  by (wpsimp wp: hoare_vcg_all_lift hoare_vcg_imp_lift' hoare_vcg_disj_lift set_sc_active_sc_tcb_at_const set_sc_budget_sufficient_const
-                    set_sc_obj_ref_budget_ready_const)
-
-(* FIXME: move *)
-lemma update_sko_sko_at_pred_indep_types:
-  "(\<forall>x y. D x \<noteq> C y) \<Longrightarrow> inj D \<Longrightarrow>
-   update_sk_obj_ref D f ref new \<lbrace>\<lambda>s. Q (sk_obj_at_pred C proj P p s)\<rbrace>"
-  apply (wpsimp wp: update_sk_obj_ref_wp)
-  apply (clarsimp simp: obj_at_def sk_obj_at_pred_def)
-  done
-
-lemma test_sc_refill_max_equiv:
-  "test_sc_refill_max scp s = sc_at_pred sc_refill_max (\<lambda>x. 0 < x) scp s"
-  unfolding test_sc_refill_max_def
-  apply (clarsimp simp: sc_at_pred_n_def obj_at_def split: option.splits)
-  apply (case_tac x2; simp)
-  done
-
-lemma set_simple_obj_ref_refill_conditions[wp]:
-  "set_ntfn_obj_ref f x v \<lbrace>is_refill_sufficient scp k\<rbrace>"
-  "set_ntfn_obj_ref f x v \<lbrace>is_refill_ready scp k\<rbrace>"
-  "set_reply_obj_ref g x v \<lbrace>is_refill_sufficient scp k\<rbrace>"
-  "set_reply_obj_ref g x v \<lbrace>is_refill_ready scp k\<rbrace>"
-  apply (wpsimp wp: update_sk_obj_ref_wp)
-  apply (clarsimp simp: is_refill_sufficient_def obj_at_def)
-  apply (wpsimp wp: update_sk_obj_ref_wp)
-  apply (clarsimp simp: is_refill_ready_def obj_at_def)
-  apply (wpsimp wp: update_sk_obj_ref_wp)
-  apply (clarsimp simp: is_refill_sufficient_def obj_at_def)
-  apply (wpsimp wp: update_sk_obj_ref_wp)
-  apply (clarsimp simp: is_refill_ready_def obj_at_def)
-  done
-
-lemma set_reply_obj_ref_sc_at_pred_n[wp]:
-  "set_reply_obj_ref update ref new \<lbrace>\<lambda>s. P (sc_at_pred_n f g h sc s)\<rbrace>"
-  by (wpsimp wp: update_sk_obj_ref_wp simp: sc_at_pred_n_def obj_at_def)
-
-lemma set_ntfn_obj_ref_valid_ep_q:
-  "set_ntfn_obj_ref f x v \<lbrace>valid_ep_q\<rbrace>"
-  apply (wpsimp simp: valid_ep_q_def2)
-  apply (wpsimp wp: hoare_vcg_all_lift hoare_vcg_imp_lift' set_tcb_pred_tcb_const hoare_vcg_disj_lift
-                    set_tcb_obj_ref_budget_ready_indep update_sko_sko_at_pred_indep_types)
-  apply (clarsimp simp: bound_sc_budget_conditions_equiv test_sc_refill_max_equiv)
-  apply (wpsimp wp: hoare_vcg_ex_lift)
-  apply (clarsimp simp: bound_sc_budget_conditions_equiv test_sc_refill_max_equiv)
-  done
-
-lemma set_reply_obj_ref_valid_ep_q:
-  "set_reply_obj_ref f x v \<lbrace>valid_ep_q\<rbrace>"
-  apply (wpsimp simp: valid_ep_q_def2)
-  apply (wpsimp wp: hoare_vcg_all_lift hoare_vcg_imp_lift' set_tcb_pred_tcb_const hoare_vcg_disj_lift
-                    set_tcb_obj_ref_budget_ready_indep update_sko_sko_at_pred_indep_types)
-  apply (clarsimp simp: bound_sc_budget_conditions_equiv test_sc_refill_max_equiv)
-  apply (wpsimp wp: hoare_vcg_ex_lift)
-  apply (clarsimp simp: bound_sc_budget_conditions_equiv test_sc_refill_max_equiv)
-  done
-
-crunches tcb_release_remove, tcb_sched_action
-  for valid_ep_q[wp]: valid_ep_q
-
-lemma sched_context_maybe_unbind_ntfn_valid_ep_q[wp]:
-  "sched_context_maybe_unbind_ntfn x41 \<lbrace>valid_ep_q :: det_state \<Rightarrow> _\<rbrace>"
-  unfolding sched_context_maybe_unbind_ntfn_def
-  by (wpsimp wp: set_sc_obj_ref_valid_ep_q_const set_ntfn_obj_ref_valid_ep_q hoare_drop_imp)
-
-lemma set_thread_state_valid_ep_q_not_in_ep_q:
-  "\<lbrace> valid_ep_q and not in_ep_q thread\<rbrace> set_thread_state thread ts \<lbrace> \<lambda>_. valid_ep_q \<rbrace>"
-  apply (wpsimp simp: set_thread_state_def set_object_def wp: get_object_wp)
-  apply (clarsimp simp: valid_ep_q_def pred_neg_def dest!: get_tcb_SomeD split: option.splits)
-  apply (drule_tac x=p in spec)
-  apply (rename_tac ko; case_tac ko; clarsimp)
-  apply (drule_tac x=t in bspec, simp)
-  apply (rule conjI, clarsimp simp: st_tcb_at_kh_if_split in_ep_q_def simple_obj_at_def)
-  apply (elim conjE disjE)
-   apply (clarsimp simp: bound_sc_tcb_at_kh_if_split  in_ep_q_def simple_obj_at_def)
-  apply (rule disjI2)
-  apply (clarsimp simp: active_sc_tcb_at_defs refill_prop_defs)
-  apply (rename_tac scp sc n)
-  apply (intro conjI, clarsimp simp: bound_sc_tcb_at_kh_if_split  in_ep_q_def simple_obj_at_def)
-  apply clarsimp
-  by (intro conjI; rule_tac x=scp in exI; fastforce)
-
-lemma in_ep_q_lift:
-  assumes A: "\<And>P R p. f \<lbrace>(\<lambda>s. (ep_at_pred R p s)) :: det_state \<Rightarrow> _\<rbrace>"
-  shows "f \<lbrace>(\<lambda>s. (in_ep_q t s)) :: det_state \<Rightarrow> _\<rbrace>"
-  unfolding  in_ep_q_def
-  by (wpsimp wp: A hoare_vcg_ex_lift)
-
-lemma not_in_ep_q_lift:
-  assumes A: "\<And>P R p. f \<lbrace>(\<lambda>s. \<not> (ep_at_pred R p s)) :: det_state \<Rightarrow> _\<rbrace>"
-  shows "f \<lbrace>(\<lambda>s. (\<not> in_ep_q t s)) :: det_state \<Rightarrow> _\<rbrace>"
-  unfolding  in_ep_q_def
-  by (wpsimp wp: A hoare_vcg_all_lift)
-
-lemma unbind_notification_valid_ep_q[wp]:
-  "unbind_notification x7  \<lbrace>valid_ep_q :: det_state \<Rightarrow> _\<rbrace>"
-  unfolding unbind_notification_def
-  by (wpsimp wp: set_tcb_obj_ref_valid_ep_q_const set_ntfn_obj_ref_valid_ep_q  hoare_drop_imp)
-
-lemma finalise_cap_valid_ipc_q:
-  "finalise_cap cap fin \<lbrace> valid_ep_q:: det_state \<Rightarrow> _\<rbrace>"
-  "finalise_cap cap fin \<lbrace> valid_ntfn_q:: det_state \<Rightarrow> _\<rbrace>"
-  sorry (* valid_ipc_qs: finalise_cap *)
-
-lemma cap_delete_valid_ipc_q:
-  "cap_delete x \<lbrace>valid_ep_q:: det_state \<Rightarrow> _\<rbrace>"
-  "cap_delete x \<lbrace>valid_ntfn_q:: det_state \<Rightarrow> _\<rbrace>"
-  unfolding cap_delete_def
-  apply (wpsimp wp: rec_del_preservation finalise_cap_valid_ipc_q preemption_point_inv)
-  apply (wpsimp wp: rec_del_preservation finalise_cap_valid_ipc_q preemption_point_inv)
-  done
-
-lemma install_tcb_cap_valid_ipc_q:
-  "install_tcb_cap x41 c d e \<lbrace>valid_ep_q:: det_state \<Rightarrow> _\<rbrace>"
-  "install_tcb_cap x41 c d e \<lbrace>valid_ntfn_q:: det_state \<Rightarrow> _\<rbrace>"
-  unfolding install_tcb_cap_def
-  apply (wpsimp wp: check_cap_inv cap_delete_valid_ipc_q)
-  apply (wpsimp wp: check_cap_inv cap_delete_valid_ipc_q)
-  done
+                                            set_tcb_obj_ref_budget_ready_const
 
 lemma rec_del_scheduler_act_sane[wp]:
-  "\<lbrace>scheduler_act_sane and valid_ep_q and valid_ntfn_q\<rbrace> rec_del call \<lbrace>\<lambda>rv. scheduler_act_sane :: det_state \<Rightarrow> _\<rbrace>"
-  by (rule_tac Q="\<lambda>_. scheduler_act_sane and valid_ep_q and valid_ntfn_q" in hoare_strengthen_post[rotated],
-      simp,
-      wpsimp wp: rec_del_preservation preemption_point_inv finalise_cap_valid_ipc_q)
+  "rec_del call \<lbrace>scheduler_act_sane :: det_state \<Rightarrow> _\<rbrace>"
+  by (wpsimp wp: rec_del_preservation preemption_point_inv)
 
 crunches cap_delete
   for simple_sched_action[wp]: "simple_sched_action :: det_state \<Rightarrow> _"
 
-crunches cap_swap_for_delete, empty_slot
-  for ct_not_queued[wp]: "ct_not_queued :: det_state \<Rightarrow> _"
-  and ct_not_in_release_q[wp]: "ct_not_in_release_q :: det_state \<Rightarrow> _"
-  and cur_sc_chargeable[wp]: "cur_sc_chargeable :: det_state \<Rightarrow> _"
-
-lemma rec_del_ct_not_queued[wp]:
-  "\<lbrace>ct_not_queued and scheduler_act_sane and valid_ntfn_q and valid_ep_q\<rbrace>
-   rec_del call
-   \<lbrace>\<lambda>_. ct_not_queued :: det_state \<Rightarrow> _\<rbrace>"
-  apply (rule hoare_strengthen_post, rule rec_del_preservation)
-  by (wpsimp wp:  preemption_point_inv' finalise_cap_valid_ipc_q)+
+lemma ct_in_state_kh_lift:
+  "f \<lbrace>\<lambda>s. pred_map P (tcb_sts_of s) (cur_thread s)\<rbrace>
+   \<Longrightarrow> f \<lbrace>\<lambda>s. ct_in_state P s\<rbrace>"
+  by (clarsimp simp: ct_in_state_kh_simp)
 
 lemma rec_del_ct_not_in_release_q[wp]:
   "rec_del call \<lbrace>ct_not_in_release_q :: det_state \<Rightarrow> _\<rbrace>"
@@ -7239,6 +6646,7 @@ crunches install_tcb_cap
 for valid_sched[wp]: "valid_sched :: det_ext state \<Rightarrow> _"
 and simple_sched_action[wp]: "simple_sched_action :: det_ext state \<Rightarrow> _"
   (wp: crunch_wps check_cap_inv simp: crunch_simps)
+
 lemma install_tcb_frame_cap_valid_sched:
   "\<lbrace>valid_sched and simple_sched_action and invs\<rbrace> install_tcb_frame_cap a d f \<lbrace>\<lambda>_. valid_sched :: det_state \<Rightarrow> _\<rbrace>"
   unfolding install_tcb_frame_cap_def
@@ -7247,8 +6655,6 @@ lemma install_tcb_frame_cap_valid_sched:
 
 
 end
-
-context DetSchedSchedule_AI begin
 
 crunch scheduler_act_not[wp]: set_priority "scheduler_act_not y"
   (wp: crunch_wps simp: crunch_simps)
@@ -7277,6 +6683,32 @@ lemma set_priority_bound_sc_tcb_at_cur_thread[wp]:
 crunch simple_sched_action[wp]: sched_context_bind_tcb simple_sched_action
   (wp: crunch_wps simp: crunch_simps)
 
+lemma set_mcpriority_bound_sc_tcb_at_cur_thread[wp]:
+  "set_mcpriority target a \<lbrace>(\<lambda>s. bound_sc_tcb_at P (cur_thread s) s)\<rbrace>"
+  unfolding set_mcpriority_def
+  apply (wpsimp simp: thread_set_def wp: set_object_wp)
+  by (clarsimp simp: pred_tcb_at_def obj_at_def dest!: get_tcb_SomeD)
+
+lemma reorder_ntfn_bound_sc_tcb_at_cur_thread[wp]:
+  "\<lbrace>\<lambda>s. bound_sc_tcb_at P (cur_thread s) s\<rbrace>
+   reorder_ntfn a
+   \<lbrace>\<lambda>_. \<lambda>s. bound_sc_tcb_at P (cur_thread s) s\<rbrace>"
+  by (rule_tac f="cur_thread" in hoare_lift_Pf; wpsimp)
+
+lemma reorder_ep_bound_sc_tcb_at_cur_thread[wp]:
+  "\<lbrace>\<lambda>s. bound_sc_tcb_at P (cur_thread s) s\<rbrace>
+   reorder_ep a
+   \<lbrace>\<lambda>_. \<lambda>s. bound_sc_tcb_at P (cur_thread s) s\<rbrace>"
+  by (rule_tac f="cur_thread" in hoare_lift_Pf; wpsimp)
+
+lemma set_scheduler_action_bound_sc_tcb_at_cur_thread[wp]:
+  "\<lbrace>\<lambda>s. bound_sc_tcb_at P (cur_thread s) s\<rbrace>
+   set_scheduler_action sched_act
+   \<lbrace>\<lambda>x s. bound_sc_tcb_at P (cur_thread s) s\<rbrace>"
+  by (rule_tac f="cur_thread" in hoare_lift_Pf; wpsimp)
+
+context DetSchedSchedule_AI_det_ext begin
+
 lemma tcc_valid_sched:
   "\<lbrace>valid_sched and invs and simple_sched_action
     and (\<lambda>s. bound_sc_tcb_at bound (cur_thread s) s)
@@ -7284,8 +6716,8 @@ lemma tcc_valid_sched:
                                       croot vroot buffer)
     and ct_active and ct_schedulable\<rbrace>
      invoke_tcb (ThreadControlCaps target slot fault_handler timeout_handler croot vroot buffer)
-   \<lbrace>\<lambda>rv. valid_sched\<rbrace>"
-  (* apply (simp add: split_def cong: option.case_cong)
+   \<lbrace>\<lambda>rv. valid_sched :: det_state \<Rightarrow> _\<rbrace>"
+  apply (simp add: split_def cong: option.case_cong)
   apply wp
        \<comment> \<open>install_tcb_cap slot 2\<close>
        apply (wpsimp wp: install_tcb_frame_cap_valid_sched)
@@ -7327,42 +6759,19 @@ lemma tcc_valid_sched:
      apply (all \<open>clarsimp simp: is_cap_simps cte_wp_at_caps_of_state\<close>)
     apply (all \<open>clarsimp simp: obj_at_def is_tcb typ_at_eq_kheap_obj cap_table_at_typ\<close>)
   by auto
- *)
-  sorry (* tc_valid_sched: wait for rebase over new work *)
-
-lemma set_irq_state_budget_conditions[wp]:
-  "set_irq_state w x \<lbrace>(\<lambda>s. P (active_sc_tcb_at t s)):: det_state \<Rightarrow> _\<rbrace>"
-  "set_irq_state w x \<lbrace>(\<lambda>s. P (budget_ready t s)):: det_state \<Rightarrow> _\<rbrace>"
-  "set_irq_state w x \<lbrace>(\<lambda>s. P (budget_sufficient t s)):: det_state \<Rightarrow> _\<rbrace>"
-  apply (wpsimp simp: set_irq_state_def)
-  apply (erule rsubst[where P=P])
-  apply (clarsimp simp: active_sc_tcb_at_defs)
-  apply (wpsimp simp: set_irq_state_def)
-  apply (erule rsubst[where P=P])
-  apply (clarsimp simp: budget_ready_defs)
-  apply (wpsimp simp: set_irq_state_def)
-  apply (erule rsubst[where P=P])
-  apply (clarsimp simp: budget_sufficient_defs)
-  done
-
-crunches empty_slot_ext, empty_slot
-  for active_sc_tcb_at[wp]: "(\<lambda>s. P (active_sc_tcb_at t s)):: det_state \<Rightarrow> _"
-  and budget_ready[wp]: "(\<lambda>s. P (budget_ready t s)):: det_state \<Rightarrow> _"
-  and budget_sufficient[wp]: "(\<lambda>s. P (budget_sufficient t s)):: det_state \<Rightarrow> _"
-  (wp:  ignore: set_irq_state)
 
 crunches cancel_all_ipc
-  for active_sc_tcb_at[wp]: "(\<lambda>s. (active_sc_tcb_at t s)):: det_state \<Rightarrow> _"
+  for active_sc_tcb_at[wp]: "(\<lambda>s. P (active_sc_tcb_at t s)):: det_state \<Rightarrow> _"
   and budget_ready[wp]: "(\<lambda>s. P (budget_ready t s)):: det_state \<Rightarrow> _"
   and budget_sufficient[wp]: "(\<lambda>s. P (budget_sufficient t s)):: det_state \<Rightarrow> _"
   (wp: crunch_wps)
 
 lemma restart_thread_if_no_fault_ct_in_state_neq:
-  "\<lbrace>ct_in_state P and (\<lambda>s. t \<noteq> cur_thread s)\<rbrace>
+  "\<lbrace>ct_in_state P and (\<lambda>s. t \<noteq> cur_thread s \<or> (P Inactive \<and> P Restart))\<rbrace>
    restart_thread_if_no_fault t
   \<lbrace>\<lambda>_. ct_in_state P :: det_state \<Rightarrow> _\<rbrace>"
   unfolding restart_thread_if_no_fault_def
-  by (wpsimp wp: sts_ctis_neq)
+  by (wpsimp wp: sts_ctis_neq simp: thread_get_def)
 
 lemma reply_unlink_tcb_ct_in_state_neq:
   "\<lbrace>ct_in_state P and (\<lambda>s. t \<noteq> cur_thread s)\<rbrace>
@@ -7370,34 +6779,6 @@ lemma reply_unlink_tcb_ct_in_state_neq:
   \<lbrace>\<lambda>_. ct_in_state P :: det_state \<Rightarrow> _\<rbrace>"
   unfolding reply_unlink_tcb_def
   by (wpsimp wp: sts_ctis_neq gts_wp get_simple_ko_wp)
-
-lemma cancel_all_ipc_ct_in_state[wp]:
-  "\<lbrace>ct_active and valid_ep_q\<rbrace>
-   cancel_all_ipc epptr
-  \<lbrace>\<lambda>_. ct_active :: det_state \<Rightarrow> _\<rbrace>"
-  unfolding cancel_all_ipc_def
-  apply wpsimp
-       apply (rule_tac I="ct_active and (\<lambda>s. \<forall>x. x \<in> set queue \<longrightarrow> x \<noteq> cur_thread s)" in mapM_x_inv_wp)
-         apply clarsimp
-        prefer 2
-        apply (assumption)
-       apply (wpsimp wp: restart_thread_if_no_fault_ct_in_state_neq gts_wp)
-      apply (wpsimp wp: restart_thread_if_no_fault_ct_in_state_neq gts_wp)
-     apply (wpsimp wp: get_ep_queue_wp)
-    apply wpsimp
-      apply (rule_tac I="ct_active and (\<lambda>s. \<forall>x. x \<in> set queue \<longrightarrow> x \<noteq> cur_thread s)" in mapM_x_inv_wp)
-        apply clarsimp
-       prefer 2
-       apply (assumption)
-      apply (wpsimp wp: restart_thread_if_no_fault_ct_in_state_neq gts_wp)
-     apply (wpsimp wp: restart_thread_if_no_fault_ct_in_state_neq gts_wp)
-    apply (wpsimp wp: get_ep_queue_wp)
-   apply (wpsimp wp: get_simple_ko_wp)
-  apply (clarsimp simp: obj_at_def)
-  apply (clarsimp simp: valid_ep_q_def)
-  apply (drule_tac x=epptr in spec)
-  apply (fastforce)
-  done
 
 lemma install_tcb_cap_active_sc_tcb_at[wp]:
   "\<lbrace>invs and tcb_at target  and active_sc_tcb_at t \<rbrace>
@@ -7420,8 +6801,8 @@ lemma install_tcb_cap_budget_sufficient[wp]:
   unfolding install_tcb_cap_def
   by (wpsimp wp: check_cap_inv cap_delete_fh_lift)
 
-lemma install_tcb_cap_ct_active[wp]:
-  "\<lbrace>invs and tcb_at target and ct_active and valid_ep_q\<rbrace>
+lemma install_tcb_cap_ct_active:
+  "\<lbrace>invs and tcb_at target and ct_active and schedulable_ipc_queues\<rbrace>
    install_tcb_cap target slot 3 slot_opt
   \<lbrace>\<lambda>_. ct_active :: det_state \<Rightarrow> _\<rbrace>"
   unfolding install_tcb_cap_def
@@ -7429,24 +6810,17 @@ lemma install_tcb_cap_ct_active[wp]:
   apply (wpsimp wp: check_cap_inv )
   apply (simp)
   apply (rule valid_validE, rule cap_delete_fh_lift)
-  apply wpsimp+
-  apply assumption
-  by clarsimp
+  by wpsimp+
 
 crunches install_tcb_cap
   for cur_thread[wp]: "(\<lambda>s. P (cur_thread s)) :: det_state \<Rightarrow> _"
   (wp: crunch_wps preemption_point_inv check_cap_inv dxo_wp_weak)
 
-lemma budget_RS_rewrite_helper:
-  "bound_sc_tcb_at (\<lambda>p. \<exists>scp. is_refill_ready scp 0 s' \<and> p = Some scp) t s' = budget_ready t s'"
-  "bound_sc_tcb_at (\<lambda>p. \<exists>scp. is_refill_sufficient scp 0 s' \<and> p = Some scp) t s' = budget_sufficient t s'"
-  by (fastforce simp: budget_ready_defs)+
-
 lemma tcs_valid_sched:
   "\<lbrace>valid_sched and invs and simple_sched_action
     and (\<lambda>s. bound_sc_tcb_at bound (cur_thread s) s)
     and tcb_inv_wf (ThreadControlSched target slot fault_handler mcp priority sc)
-    and ct_active and ct_ARS\<rbrace>
+    and ct_active and ct_schedulable\<rbrace>
      invoke_tcb (ThreadControlSched target slot fault_handler mcp priority sc)
    \<lbrace>\<lambda>rv. valid_sched :: det_state \<Rightarrow> _\<rbrace>"
   apply (simp add: split_def cong: option.case_cong)
@@ -7455,26 +6829,25 @@ lemma tcs_valid_sched:
       apply (clarsimp cong: conj_cong)
       apply (wpsimp wp: maybe_sched_context_bind_tcb_valid_sched
                         maybe_sched_context_unbind_tcb_valid_sched, assumption)
+     apply (strengthen not_cur_thread_2_simps)
      \<comment> \<open>set priority\<close>
      apply (clarsimp cong: conj_cong)
      apply (rule hoare_post_add[where R="\<lambda>_.valid_sched and simple_sched_action"])
      apply (clarsimp cong: conj_cong)
-     apply (wpsimp wp: maybeM_wp_drop_None set_priority_valid_sched hoare_vcg_all_lift hoare_vcg_imp_lift)
-      apply (wps, wpsimp)
-     apply (clarsimp, assumption)
+     apply (wp maybeM_wp_drop_None)
+     apply (wpsimp wp: set_priority_valid_sched hoare_vcg_all_lift hoare_vcg_imp_lift)
+     apply (subst conj_assoc[symmetric])+
+     apply (rule conjI, assumption, fastforce)
     \<comment> \<open>set mcpriority\<close>
     apply (wpsimp wp: maybeM_wp_drop_None)
      apply ((wpsimp wp: hoare_vcg_all_lift hoare_vcg_imp_lift
-                        set_mcpriority_budget_ready
-                        set_mcpriority_budget_sufficient
                         hoare_vcg_disj_lift
              | rule hoare_lift_Pf[where f = cur_thread])+)[1]
     apply (clarsimp, assumption)
    \<comment> \<open>install_tcb_cap\<close>
    apply (rule hoare_vcg_E_elim, wpsimp)
    apply (rule valid_validE_R)
-   apply ((wpsimp simp: budget_RS_rewrite_helper
-                    wp: hoare_vcg_disj_lift hoare_vcg_all_lift
+   apply ((wpsimp wp: hoare_vcg_disj_lift hoare_vcg_all_lift install_tcb_cap_ct_active
                         install_tcb_cap_bound_sc_tcb_at static_imp_wp
           | rule valid_validE, wps, wpsimp wp: install_tcb_cap_bound_sc_tcb_at)+)[1]
   \<comment> \<open>resolve using preconditions\<close>
@@ -7482,11 +6855,11 @@ lemma tcs_valid_sched:
   apply (intro conjI impI;
          clarsimp simp: is_cnode_or_valid_arch_is_cap_simps tcb_ep_slot_cte_wp_ats real_cte_at_cte
                  dest!: valid_vtable_root_is_arch_cap)
-     apply (erule valid_sched_implies_valid_ipc_qs)
-    apply (case_tac x; simp)
+     apply (clarsimp simp: vs_all_heap_simps tcb_at_kh_simps)
+    apply (clarsimp simp: valid_sched_def)
    apply (case_tac x; simp)
-  apply (case_tac priority; simp)
-  apply (drule valid_sched_implies_valid_ipc_qs(1), simp)
+   apply (clarsimp simp: vs_all_heap_simps tcb_at_kh_simps)
+  apply (clarsimp simp: valid_sched_def)
   done
 
 end
@@ -9904,7 +9277,6 @@ lemma sched_context_update_consumed_ko_at_Endpoint[wp]:
 lemma transfer_caps_valid_sched_misc[wp]:
   "transfer_caps info caps ep recv recv_buf \<lbrace>valid_sched_pred_strong P\<rbrace>"
   by (simp add: transfer_caps_def | wp transfer_caps_loop_pres | wpc)+
-  apply (simp add: transfer_caps_def | wp transfer_caps_loop_pres | wpc | (rule hoare_weaken_pre, wps))+
 
 lemma possible_switch_to_not_queued[wp]:
   "\<lbrace>not_queued t and scheduler_act_not t and K(target \<noteq> t)\<rbrace>
@@ -10584,14 +9956,23 @@ lemma thread_set_ep_at_pred[wp]:
   apply (clarsimp simp: simple_obj_at_def dest!: get_tcb_SomeD)
   done
 
-lemma thread_set_sc_budget_conditions[wp]:
-  "thread_set f t \<lbrace>\<lambda>s. Q (test_sc_refill_max scp s)\<rbrace>"
-  "thread_set f t \<lbrace>\<lambda>s. Q (is_refill_ready scp 0 s)\<rbrace>"
-  "thread_set f t \<lbrace>\<lambda>s. Q (is_refill_sufficient scp 0 s)\<rbrace>"
-  apply (wpsimp wp: thread_set_wp, clarsimp simp: test_sc_refill_max_def dest!: get_tcb_SomeD)
-  apply (wpsimp wp: thread_set_wp, clarsimp simp: is_refill_ready_def obj_at_def dest!: get_tcb_SomeD)
-  apply (wpsimp wp: thread_set_wp, clarsimp simp: is_refill_sufficient_def obj_at_def dest!: get_tcb_SomeD)
+(* FIXME: move *)
+lemma sc_at_tcb_update[iff]:
+  "tcb_at epptr s \<Longrightarrow>
+   scs_of_kh (kheap s(epptr \<mapsto> TCB ko)) = scs_of s"
+  by (rule map_eqI, auto simp add: vs_heap_simps obj_at_def is_tcb)
+
+lemma thread_set_valid_sched_misc[wp]:
+  "thread_set f t \<lbrace>\<lambda>s. P (consumed_time s) (cur_sc s) (cur_time s) (cur_domain s) (cur_thread s) (idle_thread s)
+          (ready_queues s) (release_queue s) (scheduler_action s) (last_machine_time_of s)
+          (sc_refill_cfgs_of s)\<rbrace>"
+  apply (wpsimp wp: thread_set_wp)
+  apply (subst sc_at_tcb_update; clarsimp simp: vs_all_heap_simps obj_at_kh_kheap_simps is_tcb)
   done
+
+lemma thread_set_test_sc_refill_max[wp]:
+  "thread_set f t \<lbrace>\<lambda>s. Q (test_sc_refill_max scp s)\<rbrace>"
+  by (wpsimp wp: thread_set_wp, clarsimp simp: test_sc_refill_max_def dest!: get_tcb_SomeD)
 
 context DetSchedSchedule_AI begin
 
@@ -11050,7 +10431,7 @@ crunch not_in_release_q[wp]: reply_remove "\<lambda>s::('state_ext state). not_i
   (wp: crunch_wps tcb_release_remove_not_in_release_q')
 
 lemma reply_unlink_tcb_ct_in_state:
-  "\<lbrace>ct_in_state test and (\<lambda>s. \<forall>t. reply_tcb_reply_at ((=) (Some t)) r s \<longrightarrow> cur_thread s \<noteq> t)\<rbrace>
+  "\<lbrace>ct_in_state test and (\<lambda>s. (\<forall>t. reply_tcb_reply_at ((=) (Some t)) r s \<longrightarrow> cur_thread s \<noteq> t \<or> test (Inactive)))\<rbrace>
    reply_unlink_tcb t r
    \<lbrace>\<lambda>_. ct_in_state test :: ('state_ext state) \<Rightarrow> _\<rbrace>"
   unfolding reply_unlink_tcb_def
@@ -11064,26 +10445,14 @@ lemma reply_remove_valid_sched_misc[wp]:
           (last_machine_time_of s) (etcbs_of s) (sc_refill_cfgs_of s)\<rbrace>"
   by (wpsimp wp: get_simple_ko_wp simp: reply_remove_def)
 
-  "\<lbrace>ct_in_state test and (\<lambda>s. \<forall>t. reply_tcb_reply_at ((=) (Some t)) r s \<longrightarrow> cur_thread s \<noteq> t)\<rbrace>
+lemma reply_remove_ct_in_state:
+  "\<lbrace>ct_in_state P and (\<lambda>s. \<forall>t. reply_tcb_reply_at ((=) (Some t)) r s \<longrightarrow> cur_thread s \<noteq> t \<or> P Inactive)\<rbrace>
      reply_remove t r
-   \<lbrace>\<lambda>_. ct_in_state test ::('state_ext state) \<Rightarrow> _\<rbrace>"
+   \<lbrace>\<lambda>_. ct_in_state P :: 'state_ext state \<Rightarrow> _\<rbrace>"
   unfolding reply_remove_def
   apply (wpsimp wp: reply_unlink_tcb_ct_in_state)
   apply (wpsimp wp: ct_in_state_thread_state_lift sched_context_donate_cur_thread
-                    hoare_vcg_imp_lift' hoare_vcg_all_lift get_simple_ko_wp)+
-  apply (auto simp: ct_in_state_def pred_tcb_at_def obj_at_def)
-  done
-
-lemma reply_remove_ct_active[wp]:
-  "\<lbrace>(\<lambda>s. ct_active s \<or> ct_idle s)
-    and (\<lambda>s. \<forall>t. reply_tcb_reply_at ((=) (Some t)) r s \<longrightarrow> cur_thread s \<noteq> t)\<rbrace>
-     reply_remove t r
-   \<lbrace>\<lambda>_ s::('state_ext state). (ct_active s \<or> ct_idle s)\<rbrace>"
-  unfolding reply_remove_def
-  apply (wpsimp wp: hoare_vcg_disj_lift)
-  apply (wpsimp wp: get_simple_ko_wp reply_unlink_tcb_ct_in_state
-         | wpsimp wp: ct_in_state_thread_state_lift
-                    hoare_vcg_imp_lift' hoare_vcg_all_lift)+
+                    hoare_vcg_imp_lift' hoare_vcg_all_lift get_simple_ko_wp | wps)+
   apply (auto simp: ct_in_state_def pred_tcb_at_def obj_at_def)
   done
 
@@ -11985,7 +11354,7 @@ lemma receive_ipc_preamble_lift:
   by (wpsimp simp: receive_ipc_preamble_def wp: assms)
 
 crunches receive_ipc_preamble
-  for cur_thread[wp]: "\<lambda>s. P (cur_thread s)"
+  for cur_thread[wp]: "(\<lambda>s. P (cur_thread s)) :: det_state \<Rightarrow> _"
   and not_queued[wp]: "not_queued thread "
   and not_in_release_q[wp]: "not_in_release_q thread"
   and scheduler_act_not[wp]: "scheduler_act_not thread"
@@ -13019,12 +12388,6 @@ lemma sched_context_yield_to_valid_sched_helper2:
 
 (* end *)
 
-lemma sched_context_resume_valid_sched_misc[wp]:
-  "sched_context_resume scp \<lbrace>\<lambda>s. P (consumed_time s) (cur_sc s) (cur_time s) (cur_domain s) (cur_thread s)
-                                   (idle_thread s) (scheduler_action s) (last_machine_time_of s) (kheap s)\<rbrace>"
-  unfolding sched_context_resume_def
-  by (wpsimp wp: hoare_drop_imp)
-
 crunches sched_context_resume
   for pred_tcb_at_ct[wp]: "\<lambda>s. pred_tcb_at P proj (cur_thread s) s"
     (wp: crunch_wps simp: crunch_simps)
@@ -13214,6 +12577,7 @@ lemma update_sched_context_not_active_sc_tcb_at:
    done
 lemma set_refills_ep_at_pred[wp]:
   "set_refills sc_ptr refills \<lbrace>\<lambda>s. Q (ep_at_pred P p s)\<rbrace>"
+  unfolding set_refills_def
   apply (wpsimp wp: update_sched_context_wp)
   apply (clarsimp simp: obj_at_def simple_obj_at_def split: if_splits)
   done
@@ -13647,23 +13011,34 @@ lemma invoke_untyped_scheduler_act_sane[wp]:
 lemma invoke_untyped_oe[wp]:
   "\<lbrace>ct_not_in_release_q\<rbrace>
    invoke_untyped x
-   -, \<lbrace>\<lambda>rv. ct_not_in_release_q :: det_state \<Rightarrow> _\<rbrace>"
+   -, \<lbrace>\<lambda>rv. ct_not_in_release_q :: 'state_ext state \<Rightarrow> _\<rbrace>"
   "\<lbrace>ct_not_queued\<rbrace>
    invoke_untyped x
-   -, \<lbrace>\<lambda>rv. ct_not_queued :: det_state \<Rightarrow> _\<rbrace>"
+   -, \<lbrace>\<lambda>rv. ct_not_queued :: 'state_ext state \<Rightarrow> _\<rbrace>"
   by (rule valid_validE_E, rule hoare_weaken_pre, wps, wpsimp, simp)+
+
+lemma update_time_stamp_schedulable_ipc_queues[wp]:
+  "\<lbrace>schedulable_ipc_queues and valid_machine_time\<rbrace>
+   update_time_stamp
+   \<lbrace>\<lambda>_. schedulable_ipc_queues :: 'state_ext state \<Rightarrow> _\<rbrace>"
+  unfolding schedulable_ipc_queues_defs schedulable_sc_tcb_at_def
+  apply (wpsimp wp: hoare_vcg_all_lift hoare_vcg_imp_lift' hoare_vcg_disj_lift update_time_stamp_budget_ready)
+  by auto
+
+end
+
+context DetSchedSchedule_AI_det_ext begin
 
 crunches cap_delete
   for scheduler_act_sane[wp]: " scheduler_act_sane :: det_state \<Rightarrow> _"
   (wp: crunch_wps simp: crunch_simps)
-lemma cap_delete_ct_not_in_release_qE_E[wp]:
+
+lemma cap_delete_ct_not_in_release_qE_E:
   "\<lbrace>ct_not_in_release_q\<rbrace>
    cap_delete x
    -, \<lbrace>\<lambda>rv. ct_not_in_release_q:: det_state \<Rightarrow> _\<rbrace>"
-  "\<lbrace>ct_not_queued and scheduler_act_sane and valid_ntfn_q and valid_ep_q\<rbrace>
-  cap_delete x
-   -, \<lbrace>\<lambda>rv. ct_not_queued:: det_state \<Rightarrow> _\<rbrace>"
-  unfolding cap_delete_def by wpsimp+
+  unfolding cap_delete_def by (wpsimp wp: )+
+
 lemma set_tcb_obj_ref_ct_in_state_no_change:
   "(\<And>y. P (tcb_state y) \<Longrightarrow> P (tcb_state (f (\<lambda>_. new) y))) \<Longrightarrow>
    set_tcb_obj_ref f ref new \<lbrace>ct_in_state P:: det_state \<Rightarrow> _\<rbrace>"
@@ -13675,16 +13050,11 @@ lemma set_tcb_obj_ref_ct_in_state_no_change:
 lemma preemption_point_ct_in_state[wp]:
   "preemption_point \<lbrace>ct_in_state P:: det_state \<Rightarrow> _\<rbrace>"
   by (wpsimp wp: preemption_point_inv; clarsimp simp: ct_in_state_def)
-lemma update_time_stamp_valid_sched_misc[wp]:
-  "update_time_stamp \<lbrace>\<lambda>s. P (cur_sc s) (cur_domain s) (cur_thread s) (idle_thread s)
-          (ready_queues s) (release_queue s) (scheduler_action s)
-          (etcbs_of s) (tcb_sts_of s) (tcb_scps_of s) (sc_refill_cfgs_of s)\<rbrace>"
-  by wpsimp
 
 crunches finalise_cap
   for ct_not_blocked[wp]: "ct_not_blocked :: det_state \<Rightarrow> _"
-  (ignore: set_tcb_obj_ref
-       wp: crunch_wps set_thread_state_ct_in_state set_tcb_obj_ref_ct_in_state_no_change thread_set_ct_in_state maybeM_inv)
+  (ignore: set_tcb_obj_ref set_object thread_set
+       wp: set_thread_state_ct_in_state crunch_wps set_tcb_obj_ref_ct_in_state_no_change thread_set_ct_in_state maybeM_inv)
 
 crunches cap_swap_ext, cap_delete
   for ct_not_blocked[wp]: "ct_not_blocked :: det_state \<Rightarrow> _"
@@ -13696,29 +13066,36 @@ lemmas rec_del_invs''_CTEDeleteCall = rec_del_invs''
                                        simplified pred_conj_def,
                                        THEN use_specE']
 
-lemma cap_delete_cur_sc_chargeable[wp]:
-  "\<lbrace>cur_sc_chargeable and ct_not_blocked and valid_ep_q and valid_ntfn_q and invs \<rbrace>
+lemma cap_delete_cur_thread_on_preemption:
+  "\<lbrace>cur_thread_on_preemption and simple_sched_action and ct_not_blocked and valid_sched and invs \<rbrace>
    cap_delete x
-   \<lbrace>\<lambda>rv. cur_sc_chargeable :: det_state \<Rightarrow> _\<rbrace>"
+   \<lbrace>\<lambda>rv. cur_thread_on_preemption :: det_state \<Rightarrow> _\<rbrace>"
   unfolding cap_delete_def
-  apply (rule_tac Q="\<lambda>_. cur_sc_chargeable and ct_not_blocked and valid_ep_q and valid_ntfn_q and invs "
-                  in hoare_strengthen_post)
-  apply (wpsimp wp: rec_del_invs''_CTEDeleteCall
-                    [where Q="cur_sc_chargeable and ct_not_blocked and valid_ep_q and valid_ntfn_q",
-                     simplified]
-                    preemption_point_inv finalise_cap_valid_ipc_q)
-  apply (clarsimp simp: ct_in_state_def)+
-lemma cap_revoke_scheduler_act_sane[wp]:
-  "\<lbrace>scheduler_act_sane and valid_ep_q and valid_ntfn_q\<rbrace>
+  apply (rule_tac Q="\<lambda>_. cur_thread_on_preemption and simple_sched_action and ct_not_blocked and valid_sched and invs "
+                   in hoare_strengthen_post)
+   apply (wpsimp wp: rec_del_invs''_CTEDeleteCall
+                     [where Q="cur_thread_on_preemption and simple_sched_action and ct_not_blocked and valid_sched",
+                      simplified])
+        apply (wpsimp simp: cur_thread_on_preemption_def)
+       apply wpsimp
+      apply (wpsimp wp: finalise_cap_cur_thread_on_preemption)
+     apply (wpsimp simp: cur_thread_on_preemption_def)
+    apply (wpsimp wp: preemption_point_inv simp: cur_thread_on_preemption_def ct_in_state_def)
+   apply (clarsimp simp: ct_in_state_def)+
+  done
+
+lemma cap_revoke_scheduler_act_sane:
+  "\<lbrace>simple_sched_action and valid_sched and ct_not_blocked and invs\<rbrace>
    cap_revoke a
   \<lbrace>\<lambda>rv. scheduler_act_sane :: det_state \<Rightarrow> _\<rbrace>"
   apply (rule hoare_strengthen_post)
    apply (rule validE_valid, rule cap_revoke_preservation)
-    apply (wpsimp wp: preemption_point_inv cap_delete_valid_ipc_q)+
+     apply (wpsimp wp: preemption_point_inv  simp: ct_in_state_def)+
+  done
 
-crunches cap_insert, sched_context_unbind_tcb, sched_context_bind_tcb, set_priority, set_mcpriority
-  for scheduler_act_sane[wp]: "scheduler_act_sane :: det_state \<Rightarrow> _"
-  (wp: crunch_wps tcb_release_remove_not_in_release_q')
+crunches install_tcb_cap
+  for ct_not_blocked[wp]: "ct_not_blocked :: det_state \<Rightarrow> _"
+  (wp: crunch_wps check_cap_inv)
 
 lemma tcb_release_enqueue_not_in_release_q:
   "\<lbrace>not_in_release_q t' and (\<lambda>s. t \<noteq> t')\<rbrace>
@@ -13727,7 +13104,7 @@ lemma tcb_release_enqueue_not_in_release_q:
   unfolding tcb_release_enqueue_def
   apply wpsimp
      apply (rule_tac Q="\<lambda>_ _. not_in_release_q_2 (qs) t' \<and> (t \<noteq> t')" in hoare_strengthen_post[rotated])
-      apply (fastforce simp: not_in_release_q_def dest: in_set_zip1)
+      apply (fastforce simp: not_in_release_q_def in_queue_2_def intro: in_set_zip1)
      apply wpsimp+
   done
 
@@ -13740,109 +13117,79 @@ lemma tcb_release_enqueue_ct_not_in_release_q[wp]:
   apply (wpsimp wp: tcb_release_enqueue_not_in_release_q)+
   done
 
-lemma postpone_ct_not_in_release_q[wp]:
-  "\<lbrace>ct_not_in_release_q and (\<lambda>s. sc_tcb_sc_at (\<lambda>x. x \<noteq> Some (cur_thread s)) x2a s)\<rbrace>
-   postpone x2a
-   \<lbrace>\<lambda>xb. ct_not_in_release_q\<rbrace>"
-  unfolding postpone_def
-  apply (wpsimp wp: get_sc_obj_ref_wp)
-  apply (clarsimp simp: sc_at_pred_n_def obj_at_def )
-  done
-
 crunches install_tcb_cap
   for scheduler_act_sane[wp]: "scheduler_act_sane :: det_state \<Rightarrow> _"
-  and ct_not_queued[wp]: "ct_not_queued :: det_state \<Rightarrow> _"
-  and ct_not_in_release_q[wp]: "ct_not_in_release_q :: det_state \<Rightarrow> _"
   (wp: crunch_wps preemption_point_inv ignore: check_cap_at simp: check_cap_at_def)
 
-lemma install_tcb_cap_cur_sc_chargeable[wp]:
-  "\<lbrace>cur_sc_chargeable and invs and ct_not_blocked and valid_ep_q and valid_ntfn_q\<rbrace>
+lemma cap_insert_cur_thread_on_preemption[wp]:
+  "\<lbrace>cur_thread_on_preemption\<rbrace>
+   cap_insert new_cap src_slot dest_slot
+   \<lbrace>\<lambda>rv. cur_thread_on_preemption :: det_state \<Rightarrow> _\<rbrace>"
+  unfolding cur_thread_on_preemption_def
+  by wpsimp
+
+lemma install_tcb_cap_cur_thread_on_preemption:
+  "\<lbrace>cur_thread_on_preemption and invs and ct_not_blocked and valid_sched and simple_sched_action\<rbrace>
    install_tcb_cap target slot n slot_opt
-   \<lbrace>\<lambda>rv. cur_sc_chargeable :: det_state \<Rightarrow> _\<rbrace>"
+   \<lbrace>\<lambda>rv. cur_thread_on_preemption :: det_state \<Rightarrow> _\<rbrace>"
   unfolding install_tcb_cap_def
-  by (wpsimp wp: check_cap_inv)
+  by (wpsimp wp: check_cap_inv cap_delete_cur_thread_on_preemption)
 
 lemma invoke_tcb_scheduler_act_sane[wp]:
-  "\<lbrace>scheduler_act_sane and valid_ep_q and valid_ntfn_q\<rbrace>
+  "\<lbrace>scheduler_act_sane\<rbrace>
    invoke_tcb x
    -, \<lbrace>\<lambda>rv. scheduler_act_sane:: det_state \<Rightarrow> _\<rbrace>"
   apply (case_tac x; simp)
          defer 7
          defer 4
          apply wpsimp+
-   apply (case_tac x82; wpsimp)
+    apply (case_tac x82; wpsimp)
   apply (wpsimp)
-  apply (wpsimp wp: hoare_drop_imps install_tcb_cap_valid_ipc_q simp: install_tcb_frame_cap_def)+
+  apply (wpsimp wp: hoare_drop_imps simp: install_tcb_frame_cap_def)+
   done
 
-lemma invoke_tcb_ct_not_in_release_q[wp]:
-  "\<lbrace>ct_not_in_release_q\<rbrace>
-   invoke_tcb x
-   -, \<lbrace>\<lambda>rv. ct_not_in_release_q:: det_state \<Rightarrow> _\<rbrace>"
-  "\<lbrace>ct_not_queued and scheduler_act_sane and valid_ntfn_q and valid_ep_q \<rbrace>
-   invoke_tcb x
-   -, \<lbrace>\<lambda>rv. ct_not_queued:: det_state \<Rightarrow> _\<rbrace>"
-  subgoal
-  apply (case_tac x; simp)
-           prefer 8
-           apply (case_tac x82; wpsimp)
-          apply (wpsimp simp: install_tcb_frame_cap_def | wpsimp wp: hoare_drop_imps)+
-  done
-  subgoal
-  apply (case_tac x; simp)
-           prefer 8
-           apply (case_tac x82; wpsimp)
-          apply (wpsimp wp: install_tcb_cap_valid_ipc_q simp: install_tcb_frame_cap_def | wpsimp wp: hoare_drop_imps)+
-  done
-  done
-
-crunches install_tcb_cap
-  for ct_not_blocked[wp]: "ct_not_blocked :: det_state \<Rightarrow> _"
-  (wp: crunch_wps check_cap_inv)
-
-lemma install_tcb_frame_cap_ctcscb:
-  "\<lbrace>invs and cur_sc_chargeable and
-            ct_not_blocked and valid_ep_q and valid_ntfn_q\<rbrace>
+lemma install_tcb_frame_cap_cur_thread_on_preemption:
+  "\<lbrace>invs and cur_thread_on_preemption and ct_not_blocked and simple_sched_action and valid_sched\<rbrace>
       install_tcb_frame_cap t sl buf
-   -, \<lbrace>\<lambda>rv. cur_sc_chargeable :: det_state \<Rightarrow> _\<rbrace>"
+   -, \<lbrace>\<lambda>rv. cur_thread_on_preemption :: det_state \<Rightarrow> _\<rbrace>"
   unfolding install_tcb_frame_cap_def
-  by wpsimp
+  by (wpsimp wp: cap_delete_cur_thread_on_preemption)
 
-lemma tcc_cur_sc_chargeable:
+lemma tcc_cur_thread_on_preemption:
   "\<lbrace>invs and tcb_inv_wf (ThreadControlCaps t sl fh th croot vroot buf)
-    and cur_sc_chargeable and ct_not_blocked
-    and valid_ep_q and valid_ntfn_q\<rbrace>
+    and cur_thread_on_preemption and ct_not_blocked and simple_sched_action
+    and valid_sched\<rbrace>
    invoke_tcb (ThreadControlCaps t sl fh th croot vroot buf)
-   -, \<lbrace>\<lambda>rv. cur_sc_chargeable :: det_state \<Rightarrow> _\<rbrace>"
+   -, \<lbrace>\<lambda>rv. cur_thread_on_preemption :: det_state \<Rightarrow> _\<rbrace>"
   supply if_cong[cong]
   apply (simp add: split_def cong: option.case_cong)
   apply wp
   \<comment> \<open>install_tcb_cap 2\<close>
-       apply (wpsimp wp: install_tcb_frame_cap_ctcscb)
+       apply (wpsimp wp: install_tcb_frame_cap_cur_thread_on_preemption)
       apply (simp)
       \<comment> \<open>install_tcb_cap 1\<close>
-      apply (rule hoare_vcg_E_elim, wp)
+      apply (rule hoare_vcg_E_elim, wp install_tcb_cap_cur_thread_on_preemption)
       apply (wpsimp wp: hoare_vcg_const_imp_lift_R hoare_vcg_all_lift_R
-                        install_tcb_cap_invs install_tcb_cap_valid_ipc_q)
+                        install_tcb_cap_invs install_tcb_cap_cur_thread_on_preemption)
      \<comment> \<open>install_tcb_cap 0\<close>
      apply (simp)
-     apply (rule hoare_vcg_E_elim, wp)
+     apply (rule hoare_vcg_E_elim, wp install_tcb_cap_cur_thread_on_preemption)
      apply ((wpsimp wp: hoare_vcg_const_imp_lift_R hoare_vcg_all_lift_R
-                        install_tcb_cap_invs install_tcb_cap_valid_ipc_q
+                        install_tcb_cap_invs install_tcb_cap_cur_thread_on_preemption
             | strengthen tcb_cap_always_valid_strg
             | wp install_tcb_cap_cte_wp_at_ep)+)[1]
     \<comment> \<open>install_tcb_cap 4\<close>
     apply (simp)
-    apply (rule hoare_vcg_E_elim, wp)
+    apply (rule hoare_vcg_E_elim, wp install_tcb_cap_cur_thread_on_preemption)
     apply ((wpsimp wp: hoare_vcg_const_imp_lift_R hoare_vcg_all_lift_R
-                       install_tcb_cap_invs install_tcb_cap_valid_ipc_q
+                       install_tcb_cap_invs install_tcb_cap_cur_thread_on_preemption
            | strengthen tcb_cap_always_valid_strg
            | wp install_tcb_cap_cte_wp_at_ep)+)[1]
    \<comment> \<open>install_tcb_cap 3\<close>
    apply (simp)
-   apply (rule hoare_vcg_E_elim, wp)
+   apply (rule hoare_vcg_E_elim, wp install_tcb_cap_cur_thread_on_preemption)
    apply ((wpsimp wp: hoare_vcg_const_imp_lift_R hoare_vcg_all_lift_R
-                      install_tcb_cap_invs install_tcb_cap_valid_ipc_q
+                      install_tcb_cap_invs install_tcb_cap_cur_thread_on_preemption
           | strengthen tcb_cap_always_valid_strg
           | wp install_tcb_cap_cte_wp_at_ep)+)[1]
   \<comment> \<open>cleanup\<close>
@@ -13857,211 +13204,142 @@ lemma tcc_cur_sc_chargeable:
      apply (all \<open>clarsimp simp: obj_at_def is_tcb typ_at_eq_kheap_obj cap_table_at_typ\<close>)
   by auto
 
-lemma invoke_tcb_cur_sc_chargeable:
-  "\<lbrace>cur_sc_chargeable and invs and tcb_inv_wf x and
-   ct_not_blocked and valid_ep_q and valid_ntfn_q\<rbrace>
+end
+
+context DetSchedSchedule_AI begin
+
+lemma invoke_domain_no_exception[wp]:
+  "\<lbrace>\<top>\<rbrace> invoke_domain thread domain -, \<lbrace>\<lambda>rv. P\<rbrace>"
+  by (wpsimp simp: invoke_domain_def)
+
+lemma arch_invoke_irq_control_ctE_E[wp]:
+  "arch_invoke_irq_control x2
+   \<lbrace>ct_not_queued and ct_not_in_release_q and cur_sc_chargeable and scheduler_act_sane:: 'state_ext state \<Rightarrow> _\<rbrace>"
+  by (wpsimp wp: hoare_vcg_conj_lift)
+
+lemma update_time_stamp_valid_sched[wp]:
+  "update_time_stamp \<lbrace>valid_sched :: 'state_ext state \<Rightarrow> _\<rbrace>"
+  by (wpsimp wp: valid_sched_lift_pre_conj[where R=valid_machine_time] simp: valid_sched_def)
+
+lemma reply_push_scheduler_act_sane[wp]:
+  "reply_push caller callee reply_ptr can_donate \<lbrace>scheduler_act_sane:: 'state_ext state \<Rightarrow> _\<rbrace>"
+  unfolding reply_push_def
+  by (wpsimp wp: hoare_drop_imp hoare_vcg_all_lift | safe)+
+
+end
+
+
+context DetSchedSchedule_AI_det_ext begin
+
+lemma invoke_tcb_cur_thread_on_preemption:
+  "\<lbrace>cur_thread_on_preemption and invs and tcb_inv_wf x and
+   ct_not_blocked and valid_sched and simple_sched_action\<rbrace>
    invoke_tcb x
-   -, \<lbrace>\<lambda>rv. cur_sc_chargeable :: det_state \<Rightarrow> _\<rbrace>"
+   -, \<lbrace>\<lambda>rv. cur_thread_on_preemption :: det_state \<Rightarrow> _\<rbrace>"
   apply (case_tac x)
   defer 5
   defer 4
     apply wpsimp+
     apply (case_tac x82; wpsimp)
-    apply (wpsimp+)[2]
-  apply (wpsimp wp: tcc_cur_sc_chargeable[simplified])
+    apply ((wpsimp wp: install_tcb_cap_cur_thread_on_preemption)+)[2]
+  apply (wpsimp wp: tcc_cur_thread_on_preemption[simplified])
   done
 
-lemma invoke_domain_no_exception[wp]:
-  "\<lbrace>\<top>\<rbrace>
-   invoke_domain x61 x62
-   -, \<lbrace>\<lambda>rv. P\<rbrace>"
-  by (wpsimp simp: invoke_domain_def)+
-
-lemma cap_revoke_ct_not_queued:
-  "\<lbrace>ct_not_queued and scheduler_act_sane and valid_ntfn_q and valid_ep_q \<rbrace>
+lemma cap_revoke_cur_thread_on_preemption:
+  "\<lbrace>cur_thread_on_preemption
+    and valid_sched and invs
+    and ct_not_blocked and simple_sched_action\<rbrace>
    cap_revoke (a, b)
-   \<lbrace>\<lambda>_. ct_not_queued :: det_state \<Rightarrow> _\<rbrace>"
-  "cap_revoke (a, b) \<lbrace>ct_not_in_release_q :: det_state \<Rightarrow> _\<rbrace>"
-  "\<lbrace>cur_sc_chargeable and invs and ct_not_blocked  and valid_ntfn_q and valid_ep_q\<rbrace>
-   cap_revoke (a, b)
-   \<lbrace>\<lambda>_. cur_sc_chargeable :: det_state \<Rightarrow> _\<rbrace>"
-  subgoal
+   \<lbrace>\<lambda>rv. cur_thread_on_preemption :: det_state \<Rightarrow> _\<rbrace>"
   apply (rule hoare_strengthen_post, rule cap_revoke_preservation2)
-  apply (wpsimp wp: preemption_point_inv cap_delete_valid_ipc_q)+
-  done
-  subgoal
-  apply (rule hoare_strengthen_post, rule cap_revoke_preservation2)
-  apply (wpsimp wp: preemption_point_inv)+
-  done
-  subgoal
-  apply (rule hoare_strengthen_post, rule cap_revoke_preservation2)
-  apply (wpsimp wp: preemption_point_inv cap_delete_valid_ipc_q)+
-  apply (clarsimp simp: ct_in_state_def)+
-  done
+    apply (wpsimp wp: preemption_point_inv cap_delete_cur_thread_on_preemption)+
+     apply (clarsimp simp: ct_in_state_def cur_thread_on_preemption_def)+
   done
 
-lemma cap_revoke_cur_thread_conditions:
-  "\<lbrace>ct_not_queued and ct_not_in_release_q
-    and cur_sc_chargeable and scheduler_act_sane
-    and valid_ntfn_q and valid_ep_q and invs and ct_not_blocked\<rbrace>
-   cap_revoke (a, b)
-   \<lbrace>\<lambda>rv. ct_not_queued and ct_not_in_release_q and cur_sc_chargeable :: det_state \<Rightarrow> _\<rbrace>"
-  apply (rule hoare_strengthen_post, rule cap_revoke_preservation2)
-    apply (wpsimp wp: preemption_point_inv cap_delete_valid_ipc_q)+
-     apply (clarsimp simp: ct_in_state_def)+
+lemma invoke_cnode_cur_thread_on_preemption:
+  "\<lbrace>cur_thread_on_preemption
+    and simple_sched_action and valid_sched and invs and ct_not_blocked\<rbrace>
+   invoke_cnode x
+   -, \<lbrace>\<lambda>rv. cur_thread_on_preemption :: det_state \<Rightarrow> _\<rbrace>"
+  supply if_split [split del]
+  apply (wpsimp wp: cap_revoke_cur_thread_on_preemption simp: invoke_cnode_def)+
+  apply (rule valid_validE_E)
+  apply (wpsimp wp: cap_delete_cur_thread_on_preemption)+
   done
 
 lemma invoke_cnode_scheduler_act_sane:
-  "\<lbrace>scheduler_act_sane and valid_ep_q and valid_ntfn_q\<rbrace>
+  "\<lbrace>simple_sched_action and valid_sched and invs and ct_not_blocked\<rbrace>
    invoke_cnode x
-   -, \<lbrace>\<lambda>rv. scheduler_act_sane:: det_state \<Rightarrow> _\<rbrace>"
-  "\<lbrace>ct_not_queued and scheduler_act_sane and valid_ntfn_q and valid_ep_q\<rbrace>
-   invoke_cnode x
-   -, \<lbrace>\<lambda>rv. ct_not_queued:: det_state \<Rightarrow> _\<rbrace>"
-  "\<lbrace>ct_not_in_release_q\<rbrace>
-   invoke_cnode x
-   -, \<lbrace>\<lambda>rv. ct_not_in_release_q:: det_state \<Rightarrow> _\<rbrace>"
-  "\<lbrace>cur_sc_chargeable and invs and ct_not_blocked and valid_ntfn_q and valid_ep_q\<rbrace>
-   invoke_cnode x
-   -, \<lbrace>\<lambda>rv. cur_sc_chargeable:: det_state \<Rightarrow> _\<rbrace>"
-  supply if_splits [split del]
-  by (wpsimp wp: cap_revoke_ct_not_queued simp: invoke_cnode_def)+
+   -, \<lbrace>\<lambda>rv. scheduler_act_sane :: det_state \<Rightarrow> _\<rbrace>"
+  supply if_split [split del]
+  by (wpsimp wp: cap_revoke_scheduler_act_sane simp: invoke_cnode_def)
 
-lemma invoke_cnode_scheduler_act_sane_new:
-  "\<lbrace>ct_not_queued and ct_not_in_release_q and cur_sc_chargeable
-    and scheduler_act_sane and valid_ntfn_q and valid_ep_q and invs and ct_not_blocked\<rbrace>
-   invoke_cnode x
-   -, \<lbrace>\<lambda>rv. ct_not_queued and ct_not_in_release_q and cur_sc_chargeable:: det_state \<Rightarrow> _\<rbrace>"
-  supply if_splits [split del]
-  apply (wpsimp wp: cap_revoke_cur_thread_conditions cap_delete_ct_not_queued simp: invoke_cnode_def)+
-  apply (rule valid_validE_E)
-  apply wpsimp+
-  done
-
-lemma invoke_irq_control_scheduler_act_sane:
-  "\<lbrace>scheduler_act_sane\<rbrace>
+lemma invoke_irq_control_cur_thread_on_preemption:
+  "\<lbrace>cur_thread_on_preemption and scheduler_act_sane\<rbrace>
    invoke_irq_control x
-   -, \<lbrace>\<lambda>rv. scheduler_act_sane:: det_state \<Rightarrow> _\<rbrace>"
-  "\<lbrace>ct_not_queued\<rbrace>
-   invoke_irq_control x
-   -, \<lbrace>\<lambda>rv. ct_not_queued:: det_state \<Rightarrow> _\<rbrace>"
-  "\<lbrace>ct_not_in_release_q\<rbrace>
-   invoke_irq_control x
-   -, \<lbrace>\<lambda>rv. ct_not_in_release_q:: det_state \<Rightarrow> _\<rbrace>"
-  "\<lbrace>cur_sc_chargeable\<rbrace>
-   invoke_irq_control x
-   -, \<lbrace>\<lambda>rv. cur_sc_chargeable:: det_state \<Rightarrow> _\<rbrace>"
-  apply (case_tac x; wpsimp)
-  apply (rule valid_validE_E, rule hoare_weaken_pre, wps, wpsimp, simp)
-  apply (case_tac x; wpsimp)
-  apply (rule valid_validE_E, rule hoare_weaken_pre, wps, wpsimp, simp)
-  apply (case_tac x; wpsimp)
-  apply (rule valid_validE_E, rule hoare_weaken_pre, wps, wpsimp, simp)
-  apply (case_tac x; wpsimp)
-  done
-
-lemma arch_invoke_irq_control_ctE_E[wp]:
-  "arch_invoke_irq_control x2
-   \<lbrace>ct_not_queued and ct_not_in_release_q and cur_sc_chargeable :: det_state \<Rightarrow> _\<rbrace>"
-  apply (wpsimp wp: hoare_vcg_conj_lift)
-     apply (rule valid_validE)
-     apply (rule hoare_lift_Pf[where f=cur_thread]; wpsimp)
-    apply (rule hoare_lift_Pf[where f=cur_thread]; wpsimp)
-   apply wpsimp
-  by simp
-
-lemma invoke_irq_control_ct_on_exception:
-  "\<lbrace>ct_not_queued and ct_not_in_release_q and cur_sc_chargeable\<rbrace>
-   invoke_irq_control x
-   -, \<lbrace>\<lambda>rv. ct_not_queued and ct_not_in_release_q and cur_sc_chargeable:: det_state \<Rightarrow> _\<rbrace>"
-  by (case_tac x; wpsimp)
-
-lemma perform_invocation_scheduler_act_sane:
-  "\<lbrace>scheduler_act_sane and valid_ep_q and valid_ntfn_q\<rbrace>
-   perform_invocation a b c iv
-   -, \<lbrace>\<lambda>rv. scheduler_act_sane:: det_state \<Rightarrow> _\<rbrace>"
-  apply (case_tac iv; simp)
-  apply (wpsimp wp: invoke_irq_control_scheduler_act_sane invoke_cnode_scheduler_act_sane)+
-  done
+   -, \<lbrace>\<lambda>rv. cur_thread_on_preemption and scheduler_act_sane:: det_state \<Rightarrow> _\<rbrace>"
+  by (case_tac x; wpsimp simp: cur_thread_on_preemption_def)
 
 lemma invs_strengthen_cur_sc_tcb_only_sym_bound:
   "cur_sc_tcb_are_bound s \<and> invs s \<Longrightarrow> cur_sc_tcb_only_sym_bound s"
   unfolding cur_sc_tcb_only_sym_bound_def cur_sc_tcb_are_bound_def
-  apply clarsimp
+  apply (clarsimp simp: tcb_at_kh_simps[symmetric] pred_tcb_at_eq_commute)
   apply (intro conjI; intro allI impI)
    apply (clarsimp simp: pred_tcb_at_def obj_at_def)
-  apply (subst (asm) sym_refs_bound_sc_tcb_iff_sc_tcb_sc_at[OF refl refl], clarsimp)
+   apply (subst (asm) sym_refs_bound_sc_tcb_iff_sc_tcb_sc_at[OF refl refl], clarsimp)
   apply (subst (asm) sym_refs_bound_sc_tcb_iff_sc_tcb_sc_at[OF refl refl], clarsimp)
   apply (clarsimp simp: sc_at_pred_n_def obj_at_def)
   done
 
-lemma perform_invocation_ct_on_exception:
-  "\<lbrace>ct_not_queued and ct_not_in_release_q and cur_sc_tcb_are_bound and
-    scheduler_act_sane and valid_ntfn_q and valid_ep_q and ct_not_blocked and invs and
+lemma perform_invocation_cur_thread_on_preemption:
+  "\<lbrace>ct_not_queued and ct_not_in_release_q and cur_sc_tcb_are_bound and simple_sched_action
+    and valid_sched and ct_not_blocked and invs and
     valid_invocation iv\<rbrace>
    perform_invocation a b c iv
-   -, \<lbrace>\<lambda>rv. ct_not_queued and ct_not_in_release_q and cur_sc_chargeable :: det_state \<Rightarrow> _\<rbrace>"
+   -, \<lbrace>\<lambda>rv. cur_thread_on_preemption and scheduler_act_sane :: det_state \<Rightarrow> _\<rbrace>"
   apply (case_tac iv; simp)
-             apply wpsimp
-              apply (strengthen strengthen_cur_sc_chargeable, wpsimp)
+             apply (wpsimp simp: cur_thread_on_preemption_def)
+              apply (strengthen strengthen_cur_sc_chargeable)
+              apply (wpsimp wp: cur_sc_chargeable_invoke_untypedE_R)
              apply (fastforce intro: invs_strengthen_cur_sc_tcb_only_sym_bound)
-            apply (wpsimp)+
-         apply (wpsimp wp: hoare_vcg_E_conj hoare_elim_pred_conjE2 invoke_tcb_cur_sc_chargeable)
-         apply (fastforce intro: invs_strengthen_cur_sc_chargeable)
-        apply (wpsimp wp: invoke_cnode_scheduler_act_sane_new)+
-     apply (fastforce intro: invs_strengthen_cur_sc_chargeable)
-    apply (wpsimp wp:  invoke_irq_control_ct_on_exception)+
-    apply (fastforce intro: invs_strengthen_cur_sc_chargeable)
-   apply (wpsimp wp:  )+
-  apply (wpsimp wp: hoare_vcg_E_conj hoare_elim_pred_conjE2)
-     apply (wpsimp wp: ct_not_queued_lift)
-    apply (wpsimp wp: ct_not_in_release_q_lift)
-   apply (strengthen strengthen_cur_sc_chargeable)
+            apply wpsimp+
+         apply (wpsimp wp: hoare_vcg_E_conj hoare_elim_pred_conjE2 invoke_tcb_cur_thread_on_preemption)
+         apply (fastforce intro: invs_strengthen_cur_sc_chargeable simp: valid_sched_def cur_thread_on_preemption_def)
+        apply wpsimp+
+      apply (wpsimp wp: invoke_cnode_cur_thread_on_preemption invoke_cnode_scheduler_act_sane)
+     apply (fastforce intro: invs_strengthen_cur_sc_chargeable simp: valid_sched_def cur_thread_on_preemption_def)
+    apply (wpsimp wp: invoke_irq_control_cur_thread_on_preemption)+
+    apply (fastforce intro: invs_strengthen_cur_sc_chargeable simp: cur_thread_on_preemption_def)
    apply wpsimp
-  apply (fastforce intro: invs_strengthen_cur_sc_tcb_only_sym_bound)
+  apply (wpsimp wp: hoare_vcg_E_conj hoare_elim_pred_conjE2 simp: cur_thread_on_preemption_def)
+  apply (fastforce intro: invs_strengthen_cur_sc_tcb_only_sym_bound strengthen_cur_sc_chargeable)
   done
 
-lemma handle_invocation_schact_saneE_E:
-  "\<lbrace>scheduler_act_sane and valid_ep_q and valid_ntfn_q\<rbrace>
+lemma handle_invocation_cur_thread_on_preemption:
+  "\<lbrace>ct_not_queued and ct_not_in_release_q and cur_sc_tcb_are_bound and simple_sched_action
+    and valid_sched and invs and ct_active\<rbrace>
    handle_invocation a b c d x
-   -, \<lbrace>\<lambda>rv. scheduler_act_sane:: det_state \<Rightarrow> _\<rbrace>"
-  unfolding handle_invocation_def syscall_def
-     by (wpsimp wp: perform_invocation_scheduler_act_sane hoare_drop_imps ct_in_state_set
-                    set_thread_state_ct_valid_ep_q set_thread_state_ct_valid_ntfn_q)
-
-lemma update_time_stamp_cur_sc_tcb_are_bound[wp]:
-  "update_time_stamp \<lbrace>cur_sc_tcb_are_bound\<rbrace>"
-  unfolding cur_sc_tcb_are_bound_def
-  by (rule hoare_weaken_pre, wps, wpsimp, simp)
-
-lemma handle_invocationE_E:
-  "\<lbrace>ct_not_queued and ct_not_in_release_q and cur_sc_tcb_are_bound and
-              scheduler_act_sane and
-              valid_ntfn_q and
-              valid_ep_q and invs and ct_active\<rbrace>
-   handle_invocation a b c d x
-   -, \<lbrace>\<lambda>rv. ct_not_queued and ct_not_in_release_q and cur_sc_chargeable:: det_state \<Rightarrow> _\<rbrace>"
+   -, \<lbrace>\<lambda>rv. cur_thread_on_preemption and scheduler_act_sane:: det_state \<Rightarrow> _\<rbrace>"
   unfolding handle_invocation_def syscall_def
   apply (simp add: handle_invocation_def ts_Restart_case_helper split_def
                    liftE_liftM_liftME liftME_def bindE_assoc)
-  apply (wpsimp wp: syscall_valid perform_invocation_ct_on_exception[simplified pred_conj_def conj_assoc]
-                    set_thread_state_ct_in_state hoare_drop_imps set_thread_state_ct_valid_ntfn_q
-                    set_thread_state_ct_valid_ep_q)
+  apply (wpsimp wp: syscall_valid perform_invocation_cur_thread_on_preemption
+                    set_thread_state_ct_in_state hoare_drop_imps set_thread_state_runnable_valid_sched)
       apply (rule validE_cases_valid, clarsimp)
       apply (subst validE_R_def[symmetric])
       apply (rule_tac Q'="\<lambda>r s.
              ct_not_queued s \<and>
              ct_not_in_release_q s \<and>
              cur_sc_tcb_are_bound s \<and>
-             scheduler_act_sane s \<and>
-             valid_ntfn_q s \<and>
+             simple_sched_action s \<and>
+             valid_sched s \<and>
              thread = cur_thread s \<and>
-             valid_ep_q s \<and>
              ct_active s \<and>
              invs s \<and> valid_invocation r s" in hoare_post_imp_R[rotated])
        apply (clarsimp)
        apply (intro conjI)
-          apply (clarsimp simp: ct_in_state_def pred_tcb_at_def obj_at_def)
+           apply (fastforce simp: ct_in_state_def runnable_eq_active)
+          apply (clarsimp simp: ct_in_state_def pred_tcb_at_def obj_at_def, fastforce)
          apply (clarsimp simp: ct_in_state_def)
         apply (clarsimp simp: ct_in_state_def pred_tcb_at_def obj_at_def)
         apply (erule if_live_then_nonz_cap_invs, assumption)
@@ -14075,61 +13353,16 @@ lemma handle_invocationE_E:
      apply wpsimp+
   done
 
-crunches create_cap, cap_insert
-  for scheduler_act_sane[wp]: "scheduler_act_sane:: det_state \<Rightarrow> _"
-  (wp: hoare_drop_imps )
-
-lemma make_arch_fault_msg_scheduler_act_sane[wp]:
-  "make_arch_fault_msg a b \<lbrace>scheduler_act_sane:: det_state \<Rightarrow> _\<rbrace>"
-  by (wpsimp | wps)+
-
-lemma reply_push_scheduler_act_sane[wp]:
-  "reply_push caller callee reply_ptr can_donate \<lbrace>scheduler_act_sane:: det_state \<Rightarrow> _\<rbrace>"
-  unfolding reply_push_def
-  by (wpsimp wp: hoare_drop_imp hoare_vcg_all_lift | safe)+
-
-crunches do_ipc_transfer
-  for scheduler_act_sane[wp]: "scheduler_act_sane:: det_state \<Rightarrow> _"
-  (wp: crunch_wps)
-
-crunches update_time_stamp
-  for scheduler_act_sane[wp]: "scheduler_act_sane:: det_state \<Rightarrow> _"
-  (wp: crunch_wps hoare_drop_imps)
-
-lemma check_budget_restart_gen:
-  "\<lbrace>P\<rbrace>
-   check_budget_restart
-   \<lbrace>\<lambda>r s. r \<longrightarrow> P (s:: det_state)\<rbrace>"
-  unfolding check_budget_restart_def check_budget_def
-  apply (wpsimp wp: hoare_vcg_if_lift2 gts_wp)
-  apply (wpsimp wp: hoare_drop_imp)+
-  done
-
-lemma handle_event_scheduler_act_sane:
-  "\<lbrace>scheduler_act_sane and valid_ep_q and valid_ntfn_q and valid_machine_time\<rbrace>
+lemma handle_event_cur_thread_on_preemption:
+  "\<lbrace>ct_not_queued and ct_not_in_release_q and cur_sc_tcb_are_bound and simple_sched_action
+    and ct_active and invs and valid_sched\<rbrace>
    handle_event e
-   -, \<lbrace>\<lambda>rv. scheduler_act_sane:: det_state \<Rightarrow> _\<rbrace>"
-  apply (case_tac e; simp)
-       apply (rename_tac syscall)
-       apply (case_tac syscall; simp)
-                 apply ((wpsimp simp: handle_send_def handle_call_def imp_conjR
-                                  wp: handle_invocation_schact_saneE_E
-                                      check_budget_restart_gen)+)[11]
-      apply wpsimp+
-  done
-
-lemma handle_event_ct_conditionsE_E:
-  "\<lbrace>ct_not_queued and ct_not_in_release_q and cur_sc_tcb_are_bound
-    and ct_active and invs and scheduler_act_sane and valid_ep_q and valid_ntfn_q and valid_machine_time\<rbrace>
-   handle_event e
-   -, \<lbrace>\<lambda>rv. ct_not_queued
-            and ct_not_in_release_q
-            and cur_sc_chargeable:: det_state \<Rightarrow> _\<rbrace>"
+   -, \<lbrace>\<lambda>rv. cur_thread_on_preemption and scheduler_act_sane :: det_state \<Rightarrow> _\<rbrace>"
   apply (case_tac e; simp)
        apply (rename_tac syscall)
        apply (case_tac syscall; simp)
                  apply (wpsimp simp: handle_send_def handle_call_def
-                                 wp: handle_invocationE_E check_budget_restart_gen)+
+                                 wp: handle_invocation_cur_thread_on_preemption check_budget_restart_true)+
   done
 
 lemma misc_cur_sc_tcb_bound[wp]:
@@ -14285,6 +13518,10 @@ crunches refill_budget_check
   for bound_sc_tcb_at[wp]: "\<lambda>s. Q (bound_sc_tcb_at P t s)"
   and sc_tcb_sc_at[wp]: "\<lambda>s. Q (sc_tcb_sc_at P t s)"
 *)
+
+end
+
+context DetSchedSchedule_AI begin
 
 lemma charge_budget_valid_sched:
   "\<lbrace>valid_sched and invs and ct_not_in_release_q and ct_not_queued and scheduler_act_sane
@@ -15899,11 +15136,6 @@ lemma handle_invocation_valid_machine_time[wp]:
   unfolding handle_invocation_def syscall_def(*
   by (wpsimp wp: hoare_drop_imp simp: lookup_cap_and_slot_def) *)
   sorry (* handle_invocation_valid_machine_time *)
- "\<lbrace>valid_machine_time and is_refill_ready scp :: 'state_ext state \<Rightarrow> _\<rbrace>
-  \<lbrace>\<lambda>_. is_refill_ready scp\<rbrace>"
-  apply (rule_tac hoare_seq_ext[OF _ gets_sp])(*
-  done *)
-  sorry (* update_time_stamp_is_refill_ready *)
 lemma handle_event_valid_machine_time[wp]:
   "handle_event e \<lbrace>valid_machine_time:: 'state_ext state \<Rightarrow> _\<rbrace>"
   apply (case_tac e; simp)
